bil_auxiliaryScript.sml
@@ -1,0 +1,229 @@
+(* ========================================================================= *)
+(* FILE          : bil_auxilairyScript.sml                                   *)
+(* DESCRIPTION   : Auxiliary lemmata used by formalisation of                *)
+(*                 BAP Intermediate Language.                                *)
+(* AUTHOR        : (c) Thomas Tuerk <tuerk@kth.se> based on previous work    *)
+(*                 by Roberto Metere, KTH - Royal Institute of Technology    *)
+(* DATE          : 2017                                                      *)
+(* ========================================================================= *)
+
+open HolKernel Parse boolLib bossLib;
+
+val _ = new_theory "bil_auxiliary";
+
+open HolKernel Parse boolLib bossLib;
+open wordsTheory bitstringTheory;
+
+
+(* -------------------------------------------------------------------------- *)
+(* List lemmata                                                               *)
+(* -------------------------------------------------------------------------- *)
+
+val LAST_FILTER_EL = store_thm ("LAST_FILTER_EL",
+  ``!P l. (FILTER P l <> []) ==> (
+          (?i. (i < LENGTH l) /\ (LAST (FILTER P l) = EL i l) /\ P (EL i l) /\
+               (!j. i < j /\ j < LENGTH l ==> ~(P (EL j l)))))``,
+GEN_TAC >> Induct >- (
+  SIMP_TAC list_ss []
+) >>
+SIMP_TAC list_ss [] >>
+CONV_TAC (RENAME_VARS_CONV ["e1"]) >>
+REPEAT STRIP_TAC >>
+Cases_on `FILTER P l = []` >| [
+  Q.EXISTS_TAC `0` >>
+  Cases_on `P e1` >> FULL_SIMP_TAC list_ss [] >>
+  REPEAT STRIP_TAC >>
+  `MEM (EL j (e1::l)) (FILTER P l)` suffices_by ASM_SIMP_TAC list_ss [] >>
+  SIMP_TAC std_ss [listTheory.MEM_FILTER] >>
+  ASM_SIMP_TAC list_ss [listTheory.MEM_EL] >>
+  Q.EXISTS_TAC `PRE j` >>
+  Cases_on `j` >> FULL_SIMP_TAC list_ss [],
+
+  FULL_SIMP_TAC list_ss [] >>
+  Q.EXISTS_TAC `SUC i` >>
+  ASM_SIMP_TAC (list_ss++boolSimps.LIFT_COND_ss) [listTheory.LAST_DEF] >>
+  REPEAT STRIP_TAC >>
+  Cases_on `j` >> FULL_SIMP_TAC list_ss [] >>
+  METIS_TAC[]
+]);
+
+
+val LENGTH_LASTN_LE = store_thm ("LENGTH_LASTN_LE",
+  ``!n l. LENGTH (LASTN n l) <= LENGTH l``,
+
+SIMP_TAC list_ss [rich_listTheory.LASTN_def,
+  listTheory.LENGTH_TAKE_EQ]);
+
+
+val dropWhile_MAP = store_thm ("dropWhile_MAP",
+  ``!P f l. dropWhile P (MAP f l) =
+            MAP f (dropWhile (P o f) l)``,
+
+GEN_TAC >> GEN_TAC >>
+Induct >> ASM_SIMP_TAC list_ss [] >>
+GEN_TAC >> COND_CASES_TAC >> (
+  SIMP_TAC list_ss []
+))
+
+val DROP_GENLIST = store_thm ("DROP_GENLIST",
+  ``!n (f:num->'a) m.
+      DROP n (GENLIST f m) =
+      GENLIST (\n'. (f (n' + n))) (m - n)``,
+Induct >- (
+  SIMP_TAC (list_ss++boolSimps.ETA_ss) []
+) >>
+GEN_TAC >> Cases >- (
+  SIMP_TAC list_ss []
+) >>
+ASM_SIMP_TAC list_ss [listTheory.GENLIST_CONS, arithmeticTheory.ADD_CLAUSES])
+
+
+val INDEX_FIND_EQ_NONE = store_thm ("INDEX_FIND_EQ_NONE",
+  ``!l i P. (INDEX_FIND i P l = NONE) <=> (~(EXISTS P l))``,
+Induct >> SIMP_TAC list_ss [listTheory.INDEX_FIND_def] >>
+REPEAT GEN_TAC >> COND_CASES_TAC >> ASM_SIMP_TAC list_ss []);
+
+
+val INDEX_FIND_EQ_SOME = store_thm ("INDEX_FIND_EQ_SOME",
+  ``!l i P j e. (INDEX_FIND i P l = SOME (j, e)) <=> (
+       (i <= j) /\ (j - i < LENGTH l) /\
+       (EL (j - i) l = e) /\ P e /\ 
+       (!j'. (i <= j' /\ j' < j) ==> ~(P (EL (j' - i) l))))``,
+
+Induct >> SIMP_TAC list_ss [listTheory.INDEX_FIND_def] >>
+REPEAT GEN_TAC >> COND_CASES_TAC >| [
+  SIMP_TAC list_ss [] >>
+  EQ_TAC >| [
+    SIMP_TAC list_ss [] >>
+    PROVE_TAC[],
+
+    STRIP_TAC >>
+    Cases_on `i < j` >| [
+      `~(P (EL (i - i) (h :: l)))` by METIS_TAC[arithmeticTheory.LESS_EQ_REFL] >>
+      FULL_SIMP_TAC list_ss [],
+
+      `i = j` by DECIDE_TAC >>
+      FULL_SIMP_TAC list_ss []
+    ]
+  ],
+
+  ONCE_ASM_REWRITE_TAC[] >>
+  EQ_TAC >> STRIP_TAC >> ASM_SIMP_TAC list_ss [] >| [
+     REPEAT STRIP_TAC >- (
+       `j - i = SUC (j - SUC i)` by DECIDE_TAC >>
+       ASM_SIMP_TAC list_ss []
+     ) >>
+     Cases_on `i = j'` >- (
+       FULL_SIMP_TAC list_ss []
+     ) >>
+     Q.PAT_X_ASSUM `!j'. _ ==> ~(P _)` (MP_TAC o Q.SPEC `j'`) >>
+     `j' - i = SUC (j' - SUC i)` by DECIDE_TAC >>
+     FULL_SIMP_TAC list_ss [],
+
+
+     Cases_on `i = j` >- (
+       FULL_SIMP_TAC list_ss []
+     ) >>
+     `j - i = SUC (j - SUC i)` by DECIDE_TAC >>
+     FULL_SIMP_TAC list_ss [] >>
+     REPEAT STRIP_TAC >>
+     Q.PAT_X_ASSUM `!j'. _ ==> ~(P _)` (MP_TAC o Q.SPEC `j'`) >>
+     `j' - i = SUC (j' - SUC i)` by DECIDE_TAC >>
+     FULL_SIMP_TAC list_ss []
+  ]
+]);
+
+
+val INDEX_FIND_EQ_SOME_0 = store_thm ("INDEX_FIND_EQ_SOME_0",
+  ``!l P j e. (INDEX_FIND 0 P l = SOME (j, e)) <=> (
+       (j < LENGTH l) /\
+       (EL j l = e) /\ P e /\ 
+       (!j'. j' < j ==> ~(P (EL j' l))))``,
+
+SIMP_TAC (std_ss++boolSimps.EQUIV_EXTRACT_ss) [INDEX_FIND_EQ_SOME] >>
+Cases_on `LENGTH l` >> SIMP_TAC std_ss []);
+
+
+
+(* -------------------------------------------------------------------------- *)
+(* Word lemmata                                                               *)
+(* -------------------------------------------------------------------------- *)
+
+val fixwidth_fixwidth_le = store_thm ("fixwidth_fixwidth_le",
+  ``!v n m. n <= m ==> (fixwidth n (fixwidth m v) = fixwidth n v)``,
+
+REPEAT STRIP_TAC >>
+`LENGTH (fixwidth m v) = m` by SIMP_TAC std_ss [length_fixwidth] >>
+FULL_SIMP_TAC list_ss [LET_DEF, fixwidth_def] >>
+REPEAT COND_CASES_TAC >| [
+  FULL_SIMP_TAC list_ss [zero_extend_def, listTheory.PAD_LEFT,
+    rich_listTheory.DROP_APPEND1, DROP_GENLIST, combinTheory.K_DEF],
+
+  FULL_SIMP_TAC list_ss [zero_extend_def, listTheory.PAD_LEFT,
+    rich_listTheory.DROP_APPEND2],
+
+  FULL_SIMP_TAC arith_ss [],
+
+  ASM_SIMP_TAC arith_ss [rich_listTheory.DROP_DROP_T]
+]);
+
+
+val w2v_word_join = store_thm ("w2v_word_join",
+``FINITE univ(:'a) /\ FINITE univ(:'b) ==>
+  !w1:'a word w2:'b word. w2v (word_join w1 w2) = (w2v w1 ++ w2v w2)``,
+
+REPEAT STRIP_TAC >>
+bitstringLib.Cases_on_v2w `w1` >>
+bitstringLib.Cases_on_v2w `w2` >>
+ASM_SIMP_TAC (list_ss++wordsLib.SIZES_ss) [w2v_v2w, fixwidth_id_imp,
+  word_join_v2w, fcpTheory.index_sum]);
+
+
+val w2v_word_concat = store_thm ("w2v_word_concat",
+``FINITE univ(:'a) /\ FINITE univ(:'b) /\ (dimindex (:'c) = dimindex (:'a) + dimindex (:'b)) ==>
+  !w1:'a word w2:'b word. w2v ((w1 @@ w2):'c word) = (w2v w1 ++ w2v w2)``,
+
+REPEAT STRIP_TAC >>
+bitstringLib.Cases_on_v2w `w1` >>
+bitstringLib.Cases_on_v2w `w2` >>
+ASM_SIMP_TAC (list_ss++wordsLib.SIZES_ss) [w2v_v2w, fixwidth_id_imp, word_concat_def,
+  word_join_v2w, fcpTheory.index_sum, w2w_def, w2n_v2w, bitTheory.MOD_2EXP_def] >>
+`v2n (v ++ v') < 2 ** (LENGTH v + LENGTH v')` by (
+  METIS_TAC[bitstringTheory.v2n_lt, listTheory.LENGTH_APPEND]
+) >>
+ASM_SIMP_TAC list_ss [n2w_v2n, w2v_v2w, fixwidth_id_imp]);
+
+
+val w2v_word_concat_SYM_REWRS = save_thm ("w2v_word_concat_SYM_REWRS",
+let
+  val words_sizes = [1,8,16,32,64]
+  val max_ws = last words_sizes
+
+  val thm_idx = LIST_CONJ (for 1 (max_ws+max_ws) (fn i => fcpLib.DIMINDEX (Arbnum.fromInt i)))
+  val thm_fin = LIST_CONJ (for 1 max_ws (fn i => fcpLib.FINITE (Arbnum.fromInt i)))
+
+  val rewr_tac = REWRITE_TAC [thm_fin, thm_idx];
+
+  val thm0 = GSYM w2v_word_concat
+  fun inst_w2v_word_concat n m = let
+    val n_ty = fcpLib.index_type (Arbnum.fromInt n);
+    val m_ty = fcpLib.index_type (Arbnum.fromInt m);
+    val nm_ty = fcpLib.index_type (Arbnum.fromInt (n+m));
+
+    val thm1a = INST_TYPE [``:'a`` |-> n_ty, ``:'b`` |-> m_ty, ``:'c`` |-> nm_ty] thm0
+    val (pre, _) = dest_imp (concl(thm1a))
+    val pre_thm = prove (pre, rewr_tac >> DECIDE_TAC)
+    val thm1 = MP thm1a pre_thm
+  in thm1 end
+
+  fun words_sizes_combs_n s c = (if (c+s) <= max_ws then (s, c)::(c,s)::words_sizes_combs_n s (c+s) else [])
+  val words_sizes_combs = flatten (map (fn n => words_sizes_combs_n n n) words_sizes)
+
+  val thm1 = LIST_CONJ (map (fn (n, m) => inst_w2v_word_concat m n) words_sizes_combs)
+in
+  thm1
+end)
+
+
+val _ = export_theory();
+
