bil_envScript.sml
@@ -1,0 +1,102 @@
+(* ========================================================================= *)
+(* FILE          : bil_mem_expScript.sml                                     *)
+(* DESCRIPTION   : A model of bil variable invironments                      *)
+(* AUTHOR        : (c) Thomas Tuerk <tuerk@kth.se> based on previous work    *)
+(*                 by Roberto Metere, KTH - Royal Institute of Technology    *)
+(* DATE          : 2017                                                      *)
+(* ========================================================================= *)
+
+open HolKernel Parse boolLib bossLib;
+open wordsTheory bitstringTheory;
+open finite_mapTheory;
+open bil_auxiliaryTheory bil_immTheory bil_valuesTheory;
+
+val _ = new_theory "bil_env";
+
+val _ = Datatype `bil_var_t = Var string bil_type_t`;
+
+val bil_var_name_def = Define `bil_var_name (Var n _) = n`;
+val bil_var_type_def = Define `bil_var_type (Var _ ty) = ty`;
+
+val _ = Datatype `bil_var_environment_t =
+    IrregularEnv
+  | RegularEnv (string |-> (bil_type_t # (bil_val_t option)))`;
+
+
+(* Empty environment *)
+val empty_env_def = Define `empty_env = RegularEnv FEMPTY`
+
+val is_env_regular_def = Define `
+  (is_env_regular IrregularEnv = F) /\
+  (is_env_regular (RegularEnv _) = T)`;
+
+val is_valid_env_def = Define `(is_valid_env IrregularEnv = F) /\
+  (is_valid_env (RegularEnv m) <=> FEVERY (\ (_, (ty, vo)).
+     (case vo of NONE => T | SOME v => (ty = type_of_bil_val v))) m)`
+
+val is_valid_env_empty = store_thm ("is_valid_env_empty",
+  ``is_valid_env empty_env``,
+SIMP_TAC std_ss [is_valid_env_def, empty_env_def, finite_mapTheory.FEVERY_FEMPTY]);
+
+val is_env_regular_REWRS = store_thm ("is_env_regular_REWRS",
+``!env. is_env_regular env <=> (env <> IrregularEnv)``,
+Cases >> SIMP_TAC (srw_ss()) [is_env_regular_def])
+
+val bil_env_lookup_def = Define `
+  (bil_env_lookup varname IrregularEnv = NONE) /\
+  (bil_env_lookup varname (RegularEnv env) = FLOOKUP env varname)`
+
+val bil_env_update_def = Define `
+  (bil_env_update varname vo ty IrregularEnv = IrregularEnv) /\
+  (bil_env_update varname vo ty (RegularEnv env) = 
+    if (?v. (vo = SOME v) /\ (ty <> type_of_bil_val v)) then IrregularEnv else
+    (RegularEnv (env |+ (varname, (ty, vo)))))`;
+
+
+val bil_env_lookup_type_def = Define `
+  bil_env_lookup_type var_name env = OPTION_MAP FST (bil_env_lookup var_name env)`;
+
+val bil_env_check_type_def = Define `
+  bil_env_check_type var env = 
+    (bil_env_lookup_type (bil_var_name var) env = SOME (bil_var_type var))`
+
+
+val bil_env_read_def = Define `bil_env_read v env =
+  case (bil_env_lookup (bil_var_name v) env) of
+     NONE => Unknown
+   | SOME (_, NONE) => Unknown
+   | SOME (ty, SOME r) => if (ty = bil_var_type v) then r else Unknown`;
+
+
+val bil_env_write_def = Define `bil_env_write v va env =
+  if (bil_env_check_type v env) then bil_env_update (bil_var_name v) (SOME va) (bil_var_type v) env else IrregularEnv`;
+
+
+val bil_env_write_Irregular = store_thm ("bil_env_write_Irregular",
+  ``!v va. (bil_env_write v va IrregularEnv) = IrregularEnv``,
+SIMP_TAC std_ss [bil_env_write_def, bil_env_update_def]);
+
+val bil_env_write_Irregular_WrongVal = store_thm ("bil_env_write_Irregular_WrongVal",
+  ``!v va env. (type_of_bil_val va <> bil_var_type v) ==>
+               (bil_env_write v va env = IrregularEnv)``,
+
+REPEAT GEN_TAC >>
+SIMP_TAC std_ss [bil_env_write_def, bil_env_check_type_def] >>
+COND_CASES_TAC >> REWRITE_TAC[] >>
+Cases_on `env` >> SIMP_TAC std_ss [bil_env_update_def])
+
+
+val bil_env_var_is_bound_def = Define `
+  (bil_env_var_is_bound var IrregularEnv = F) /\
+  (bil_env_var_is_bound var (RegularEnv env) = (var IN FDOM env))` 
+
+
+val bin_env_var_is_bound_ALT_DEF = store_thm ("bin_env_var_is_bound_ALT_DEF",
+  ``!var env. bil_env_var_is_bound var env <=> IS_SOME (bil_env_lookup_type var env)``,
+
+Cases_on `env` >> (
+  SIMP_TAC (std_ss++boolSimps.LIFT_COND_ss) [bil_env_var_is_bound_def, bil_env_var_is_bound_def,
+    bil_env_lookup_type_def, bil_env_lookup_def, FLOOKUP_DEF]
+));
+
+val _ = export_theory();
