bil_expScript.sml
@@ -1,0 +1,421 @@
+(* ========================================================================= *)
+(* FILE          : bil_mem_expScript.sml                                     *)
+(* DESCRIPTION   : A model of expressions                                    *)
+(* AUTHOR        : (c) Thomas Tuerk <tuerk@kth.se> based on previous work    *)
+(*                 by Roberto Metere, KTH - Royal Institute of Technology    *)
+(* DATE          : 2017                                                      *)
+(* ========================================================================= *)
+
+open HolKernel Parse boolLib bossLib;
+open wordsTheory bitstringTheory;
+open bil_auxiliaryTheory bil_immTheory bil_valuesTheory;
+open bil_imm_expTheory bil_mem_expTheory bil_envTheory;
+
+val _ = new_theory "bil_exp";
+
+val bil_imm_ss = rewrites ((type_rws ``:bil_imm_t``) @ (type_rws ``:bil_immtype_t``));
+val bil_type_ss = rewrites ((type_rws ``:bil_type_t``));
+
+
+(* ------------------------------------------------------------------------- *)
+(*  Datatypes                                                                *)
+(* ------------------------------------------------------------------------- *)
+
+val _ = Datatype `bil_exp_t =
+    Const             bil_imm_t
+  | Den               bil_var_t
+
+  | Cast              bil_cast_t bil_exp_t bil_immtype_t
+
+  | UnaryExp          bil_unary_exp_t bil_exp_t
+  | BinExp            bil_bin_exp_t bil_exp_t bil_exp_t
+  | BinPred           bil_bin_pred_t bil_exp_t bil_exp_t
+
+    (* For some reason if-then-else officially misses in BAP documentation *)
+  | IfThenElse        bil_exp_t bil_exp_t bil_exp_t
+
+  | Load              bil_exp_t bil_exp_t bil_endian_t bil_immtype_t
+  | Store             bil_exp_t bil_exp_t bil_endian_t bil_exp_t
+`;
+
+
+(* ------------------------------------------------------------------------- *)
+(*  Semantics of expressions                                                 *)
+(* ------------------------------------------------------------------------- *)
+
+val bil_eval_cast_def = Define `
+  (bil_eval_cast ct (Imm bi) ty = Imm (bil_gencast ct bi ty)) /\
+  (bil_eval_cast _ _ _ = Unknown)`;
+
+val bil_eval_unary_exp_def = Define `
+  (bil_eval_unary_exp et (Imm bi) = Imm (bil_unary_exp et bi)) /\
+  (bil_eval_unary_exp _ _ = Unknown)`;
+
+val bil_eval_bin_exp_def = Define `
+  (bil_eval_bin_exp et (Imm bi1) (Imm bi2) =
+     if (type_of_bil_imm bi1 <> type_of_bil_imm bi2) then Unknown else
+     Imm (bil_bin_exp et bi1 bi2)) /\
+  (bil_eval_bin_exp _ _ _ = Unknown)`;
+
+val bil_eval_bin_pred_def = Define `
+  (bil_eval_bin_pred pt (Imm bi1) (Imm bi2) =
+     if (type_of_bil_imm bi1 <> type_of_bil_imm bi2) then Unknown else
+     Imm (bool2b (bil_bin_pred pt bi1 bi2))) /\
+  (bil_eval_bin_pred _ _ _ = Unknown)`;
+
+val bil_eval_ifthenelse_def = Define `
+  (bil_eval_ifthenelse (Imm (Imm1 cw)) e1 e2 =
+     if (cw = 1w) then e1 else e2) /\
+  (bil_eval_ifthenelse _ _ _ = Unknown)`;
+
+val bil_eval_load_def = Define `
+  (bil_eval_load (Mem ta tv mmap) (Imm a) en t =
+     if ((type_of_bil_imm a) = ta) then
+        (case (bil_load_from_mem tv t mmap en (b2n a)) of
+           NONE => Unknown
+         | SOME i => Imm i)
+     else Unknown) /\
+  (bil_eval_load _ _ _ _ = Unknown)`;
+
+val bil_eval_store_def = Define `
+  (bil_eval_store (Mem ta tv mmap) (Imm a) en (Imm v) =
+     if ((type_of_bil_imm a) = ta) then
+        (case (bil_store_in_mem tv v mmap en (b2n a)) of
+           NONE => Unknown
+         | SOME mmap' => Mem ta tv mmap')
+     else Unknown) /\
+  (bil_eval_store _ _ _ _ = Unknown)`;
+
+
+
+val bil_eval_exp_def = Define `
+  (bil_eval_exp (Const n) env = Imm n) /\
+
+  (bil_eval_exp (Den v) env = bil_env_read v env) /\
+
+  (bil_eval_exp (Cast ct e ty) env = (
+     bil_eval_cast ct (bil_eval_exp e env) ty)) /\
+
+  (bil_eval_exp (UnaryExp et e) env = (
+     bil_eval_unary_exp et (bil_eval_exp e env))) /\
+
+  (bil_eval_exp (BinExp et e1 e2) env = (
+     bil_eval_bin_exp et (bil_eval_exp e1 env) (bil_eval_exp e2 env))) /\
+
+  (bil_eval_exp (BinPred pt e1 e2) env = (
+     bil_eval_bin_pred pt (bil_eval_exp e1 env) (bil_eval_exp e2 env))) /\
+
+  (bil_eval_exp (IfThenElse c et ef) env =
+     bil_eval_ifthenelse (bil_eval_exp c env) (bil_eval_exp et env) (bil_eval_exp ef env)
+  ) /\
+
+  (bil_eval_exp (Load mem_e a_e en ty) env =
+     bil_eval_load (bil_eval_exp mem_e env) (bil_eval_exp a_e env) en ty) /\
+
+  (bil_eval_exp (Store mem_e a_e en v_e) env =
+     bil_eval_store (bil_eval_exp mem_e env) (bil_eval_exp a_e env) en (bil_eval_exp v_e env))
+`;
+
+
+
+
+(* ------------------------------------------------------------------------- *)
+(*  Rewrite theorems for eval                                                *)
+(* ------------------------------------------------------------------------- *)
+
+val bil_eval_cast_REWRS = store_thm ("bil_eval_cast_REWRS",
+``(!ct bi ty. (bil_eval_cast ct (Imm bi) ty = Imm (bil_gencast ct bi ty))) /\
+  (!ct ty. bil_eval_cast ct Unknown ty = Unknown) /\
+  (!ct at vt mmap ty. bil_eval_cast ct (Mem at vt mmap) ty = Unknown)``,
+SIMP_TAC std_ss [bil_eval_cast_def]);
+
+val bil_eval_unary_exp_REWRS = store_thm ("bil_eval_unary_exp_REWRS",
+ ``(!et bi. (bil_eval_unary_exp et (Imm bi) = Imm (bil_unary_exp et bi))) /\
+   (!et. bil_eval_unary_exp et Unknown = Unknown) /\
+   (!et at vt mmap. bil_eval_unary_exp et (Mem at vt mmap) = Unknown)``,
+SIMP_TAC std_ss [bil_eval_unary_exp_def]);
+
+
+val bil_eval_bin_exp_REWRS = store_thm ("bil_eval_bin_exp_REWRS",
+``(!et bi1 bi2. bil_eval_bin_exp et (Imm bi1) (Imm bi2) =
+     if (type_of_bil_imm bi1 <> type_of_bil_imm bi2) then Unknown else
+     Imm (bil_bin_exp et bi1 bi2)) /\
+  (!et v. bil_eval_bin_exp et Unknown v = Unknown) /\
+  (!et v. bil_eval_bin_exp et v Unknown = Unknown) /\
+  (!et at vt mmap v. bil_eval_bin_exp et (Mem at vt mmap) v = Unknown) /\
+  (!et at vt mmap v. bil_eval_bin_exp et v (Mem at vt mmap) = Unknown)``,
+SIMP_TAC std_ss [bil_eval_bin_exp_def] >>
+CONJ_TAC >| [
+  Cases_on `v` >> SIMP_TAC std_ss [bil_eval_bin_exp_def],
+  Cases_on `v` >> SIMP_TAC std_ss [bil_eval_bin_exp_def]
+]);
+
+val bil_eval_bin_pred_REWRS = store_thm ("bil_eval_bin_pred_REWRS",
+``(!et bi1 bi2. bil_eval_bin_pred et (Imm bi1) (Imm bi2) =
+     if (type_of_bil_imm bi1 <> type_of_bil_imm bi2) then Unknown else
+     Imm (bool2b (bil_bin_pred et bi1 bi2))) /\
+  (!et v. bil_eval_bin_pred et Unknown v = Unknown) /\
+  (!et v. bil_eval_bin_pred et v Unknown = Unknown) /\
+  (!et at vt mmap v. bil_eval_bin_pred et (Mem at vt mmap) v = Unknown) /\
+  (!et at vt mmap v. bil_eval_bin_pred et v (Mem at vt mmap) = Unknown)``,
+SIMP_TAC std_ss [bil_eval_bin_pred_def] >>
+CONJ_TAC >| [
+  Cases_on `v` >> SIMP_TAC std_ss [bil_eval_bin_pred_def],
+  Cases_on `v` >> SIMP_TAC std_ss [bil_eval_bin_pred_def]
+]);
+
+val bil_eval_ifthenelse_REWRS = store_thm ("bil_eval_ifthenelse_REWRS",
+``(!c e1 e2. bil_eval_ifthenelse (Imm c) e1 e2 =
+     if (type_of_bil_imm c = Bit1) then (
+       if (c = Imm1 1w) then e1 else e2
+     ) else Unknown) /\
+  (!c e1 e2. bil_eval_ifthenelse Unknown e1 e2 = Unknown) /\
+  (!at vt mmap e1 e2. bil_eval_ifthenelse (Mem at vt mmap) e1 e2 = Unknown)``,
+SIMP_TAC std_ss [bil_eval_ifthenelse_def] >>
+Cases_on `c` >> (
+  SIMP_TAC (std_ss++bil_imm_ss) [type_of_bil_imm_def, bil_eval_ifthenelse_def]
+));
+
+val bil_eval_ifthenelse_TF_EQ = store_thm ("bil_eval_ifthenelse_TF_EQ",
+``!c e.
+     bil_eval_ifthenelse c e e =
+     if (type_of_bil_val c = ImmType Bit1) then e else Unknown``,
+Cases_on `c` >> (
+  SIMP_TAC (std_ss++bil_imm_ss++bil_type_ss) [type_of_bil_imm_def, bil_eval_ifthenelse_REWRS,
+    type_of_bil_val_def]
+));
+
+
+val bil_eval_load_Unkown_REWRS1 = prove (
+  ``(!mem en t. bil_eval_load mem Unknown en t = Unknown) /\
+    (!mem en t aty vty mmap. bil_eval_load mem (Mem aty vty mmap) en t = Unknown)``,
+
+SIMP_TAC std_ss [bil_eval_load_def] >>
+REPEAT CONJ_TAC >>
+Cases_on `mem` >> SIMP_TAC std_ss [bil_eval_load_def]);
+
+val bil_eval_load_Unkown_REWRS2 = prove (
+  ``(!a en t. bil_eval_load Unknown a en t = Unknown) /\
+    (!a en t i. bil_eval_load (Imm i) a en t = Unknown)``,
+
+SIMP_TAC std_ss [bil_eval_load_def]);
+
+val bil_eval_load_Unkown_REWRS3 = prove (
+  ``!a en t i aty vty mmap.
+      (type_of_bil_imm i <> aty) ==>
+      (bil_eval_load (Mem aty vty mmap) (Imm i) en t = Unknown)``,
+
+SIMP_TAC std_ss [bil_eval_load_def]);
+
+
+val bil_eval_load_Unkown_REWRS4 = prove (
+  ``!a en t i aty vty mmap.
+      (t <> vty) ==>
+      (bil_eval_load (Mem aty vty mmap) (Imm i) NoEndian t = Unknown)``,
+
+SIMP_TAC std_ss [bil_eval_load_def] >>
+REPEAT STRIP_TAC >>
+COND_CASES_TAC >> SIMP_TAC std_ss [] >>
+ASM_SIMP_TAC std_ss [bil_load_from_mem_NO_ENDIAN]);
+
+val bil_eval_load_Unkown_REWRS5 = prove (
+  ``!a en t i aty vty mmap en.
+      (bil_number_of_mem_splits vty t = NONE) ==>
+      (bil_eval_load (Mem aty vty mmap) (Imm i) en t = Unknown)``,
+
+SIMP_TAC std_ss [bil_eval_load_def] >>
+REPEAT STRIP_TAC >>
+COND_CASES_TAC >> SIMP_TAC std_ss [] >>
+ASM_SIMP_TAC std_ss [bil_load_from_mem_def]);
+
+
+val bil_eval_load_Unkown_REWRS = save_thm ("bil_eval_load_Unkown_REWRS",
+  REWRITE_RULE [GSYM CONJ_ASSOC] (
+  LIST_CONJ [bil_eval_load_Unkown_REWRS1, bil_eval_load_Unkown_REWRS2, bil_eval_load_Unkown_REWRS3,
+             bil_eval_load_Unkown_REWRS4, bil_eval_load_Unkown_REWRS5]));
+
+
+val bil_eval_load_SINGLE_REWR = store_thm ("bil_eval_load_SINGLE_REWR",
+  ``!a en t i aty vty mmap en.
+      (bil_eval_load (Mem aty vty mmap) (Imm i) en vty) =
+      ((if (type_of_bil_imm i = aty) then (Imm (n2bs (mmap (b2n i)) vty))
+       else Unknown))``,
+
+SIMP_TAC arith_ss [bil_eval_load_def, bil_load_from_mem_SINGLE]);
+
+
+val bil_eval_load_BASIC_REWR = store_thm ("bil_eval_load_BASIC_REWR",
+  ``!a en t i aty vty ty mmap en.
+      (bil_eval_load (Mem aty vty mmap) (Imm i) en ty) =
+      (if type_of_bil_imm i = aty then
+        case bil_load_from_mem vty ty mmap en (b2n i) of
+          NONE => Unknown
+        | SOME i => Imm i
+       else Unknown)``,
+SIMP_TAC arith_ss [bil_eval_load_def]);
+
+
+val bil_eval_load_FULL_REWRS = save_thm ("bil_eval_load_FULL_REWRS",
+let
+  val thm_prune0 = prove (``(!ta a.
+      (type_of_bil_imm a <> ta) ==>
+      (bil_eval_load (Mem ta tv mmap) (Imm a) en tr = Unknown)) /\
+      (!tr tv.
+      (tr <> tv) ==> (bil_number_of_mem_splits tv tr <> NONE) ==>
+      (bil_eval_load (Mem ta tv mmap) (Imm i) NoEndian tr = Unknown)) /\
+      (!tr tv.
+      (bil_number_of_mem_splits tv tr = NONE) ==>
+      (bil_eval_load (Mem ta tv mmap) (Imm i) en tr = Unknown))``,
+   SIMP_TAC std_ss [bil_eval_load_Unkown_REWRS])
+
+  val thm_prune1 = SIMP_RULE (std_ss ++ bil_imm_ss ++ DatatypeSimps.expand_type_quants_ss [``:bil_immtype_t``, ``:bil_imm_t``]) [bil_number_of_mem_splits_REWRS, type_of_bil_imm_def] thm_prune0
+
+  val thm_prune2 = SIMP_RULE std_ss [FORALL_AND_THM, GSYM CONJ_ASSOC] (GEN_ALL thm_prune1)
+
+
+  val thm0 = bil_eval_load_BASIC_REWR
+
+  val thm1 = SIMP_RULE (list_ss ++ bil_imm_ss ++ DatatypeSimps.expand_type_quants_ss [``:bil_immtype_t``, ``:bil_imm_t``, ``:bil_endian_t``]) [ type_of_bil_imm_def, size_of_bil_immtype_def, bil_number_of_mem_splits_REWRS, bil_load_from_mem_REWRS, thm_prune2]
+     thm0
+
+  val thm2 = Ho_Rewrite.REWRITE_RULE [fold_bil_endian_THM] thm1
+
+  val thm3 = SIMP_RULE (list_ss) [
+     FORALL_AND_THM, b2n_MOD_2EXP, type_of_bil_imm_def, size_of_bil_immtype_def]
+     thm2
+
+  val thm4 = REWRITE_RULE [b2n_def, GSYM CONJ_ASSOC] (CONJ thm3 thm_prune2)
+in thm4
+end);
+
+val bil_eval_store_Unkown_REWRS1 = prove (
+  ``(!mem en v. bil_eval_store mem Unknown en v = Unknown) /\
+    (!mem en v aty vty mmap. bil_eval_store mem (Mem aty vty mmap) en v = Unknown)``,
+
+SIMP_TAC std_ss [bil_eval_store_def] >>
+REPEAT CONJ_TAC >>
+Cases_on `mem` >> SIMP_TAC std_ss [bil_eval_store_def]);
+
+val bil_eval_store_Unkown_REWRS2 = prove (
+  ``(!a en v. bil_eval_store Unknown a en v = Unknown) /\
+    (!a en v i. bil_eval_store (Imm i) a en v = Unknown)``,
+
+SIMP_TAC std_ss [bil_eval_store_def]);
+
+
+val bil_eval_store_Unkown_REWRS3 = prove (
+  ``(!a en mem. bil_eval_store mem a en Unknown = Unknown) /\
+    (!a en mem ta tv mmap. bil_eval_store mem a en (Mem ta tv mmap) = Unknown)``,
+
+REPEAT CONJ_TAC >>
+Cases_on `mem` >> Cases_on `a` >> SIMP_TAC std_ss [bil_eval_store_def]);
+
+
+val bil_eval_store_Unkown_REWRS4 = prove (
+  ``!en v i aty vty mmap.
+      (type_of_bil_imm i <> aty) ==>
+      (bil_eval_store (Mem aty vty mmap) (Imm i) en v = Unknown)``,
+Cases_on `v` >>
+SIMP_TAC std_ss [bil_eval_store_def]);
+
+
+val bil_eval_store_Unkown_REWRS5 = prove (
+  ``!a en v aty vty mmap.
+      (type_of_bil_imm v <> vty) ==>
+      (bil_eval_store (Mem aty vty mmap) a NoEndian (Imm v) = Unknown)``,
+
+Cases_on `a` >> SIMP_TAC std_ss [bil_eval_store_def] >>
+REPEAT STRIP_TAC >>
+COND_CASES_TAC >> SIMP_TAC std_ss [] >>
+ASM_SIMP_TAC std_ss [bil_store_in_mem_NO_ENDIAN]);
+
+
+val bil_eval_store_Unkown_REWRS6 = prove (
+  ``!a en v aty vty mmap en.
+      (bil_number_of_mem_splits vty (type_of_bil_imm v) = NONE) ==>
+      (bil_eval_store (Mem aty vty mmap) a en (Imm v) = Unknown)``,
+
+Cases_on `a` >> SIMP_TAC std_ss [bil_eval_store_def, LET_DEF] >>
+REPEAT STRIP_TAC >>
+COND_CASES_TAC >> SIMP_TAC std_ss [] >>
+ASM_SIMP_TAC std_ss [bil_store_in_mem_def, LET_DEF]);
+
+
+val bil_eval_store_Unkown_REWRS = save_thm ("bil_eval_store_Unkown_REWRS",
+  SIMP_RULE std_ss [GSYM CONJ_ASSOC] (
+  LIST_CONJ [bil_eval_store_Unkown_REWRS1, bil_eval_store_Unkown_REWRS2, bil_eval_store_Unkown_REWRS3,
+             bil_eval_store_Unkown_REWRS4, bil_eval_store_Unkown_REWRS5, bil_eval_store_Unkown_REWRS6]));
+
+val bil_eval_store_SINGLE_REWR = store_thm ("bil_eval_store_SINGLE_REWR",
+  ``!a en t i aty v vty mmap en.
+      ((type_of_bil_imm i = aty) /\ (type_of_bil_imm v = vty)) ==>
+      (bil_eval_store (Mem aty vty mmap) (Imm i) en (Imm v) =
+      (Mem aty vty ((b2n i =+ b2n v) mmap)))``,
+
+SIMP_TAC arith_ss [bil_eval_store_def, bil_store_in_mem_SINGLE]);
+
+
+
+val bil_eval_store_BASIC_REWR = store_thm ("bil_eval_store_BASIC_REWR",
+  ``!a en t i aty v vty mmap en.
+      (bil_eval_store (Mem aty vty mmap) (Imm i) en (Imm v) =
+      (if type_of_bil_imm i = aty then
+         case bil_store_in_mem vty v mmap en (b2n i) of
+           NONE => Unknown
+         | SOME mmap' => Mem aty vty mmap'
+       else Unknown))``,
+
+SIMP_TAC arith_ss [bil_eval_store_def]);
+
+
+val bil_eval_store_FULL_REWRS = save_thm ("bil_eval_store_FULL_REWRS",
+let
+  val thm_prune0 = prove (``(!ta a.
+      (type_of_bil_imm a <> ta) ==>
+      (bil_eval_store (Mem ta tv mmap) (Imm a) en v = Unknown)) /\
+      (!i tv.
+      (type_of_bil_imm i <> tv) ==> (bil_number_of_mem_splits tv (type_of_bil_imm i) <> NONE) ==>
+      (bil_eval_store (Mem ta tv mmap) a NoEndian (Imm i) = Unknown)) /\
+      (!i tv.
+      (bil_number_of_mem_splits tv (type_of_bil_imm i) = NONE) ==>
+      (bil_eval_store (Mem ta tv mmap) a en (Imm i) = Unknown))``,
+   SIMP_TAC std_ss [bil_eval_store_Unkown_REWRS])
+
+  val thm_prune1 = SIMP_RULE (std_ss ++ bil_imm_ss ++ DatatypeSimps.expand_type_quants_ss [``:bil_immtype_t``, ``:bil_imm_t``]) [bil_number_of_mem_splits_REWRS, type_of_bil_imm_def] thm_prune0
+
+  val thm_prune2 = SIMP_RULE std_ss [FORALL_AND_THM, GSYM CONJ_ASSOC] (GEN_ALL thm_prune1)
+
+
+  val thm0 = SIMP_RULE (std_ss) [bil_eval_store_Unkown_REWRS, FORALL_AND_THM] bil_eval_store_BASIC_REWR
+
+  val thm1 = SIMP_RULE (list_ss++ bil_imm_ss ++ DatatypeSimps.expand_type_quants_ss [``:bil_immtype_t``, ``:bil_imm_t``, ``:bil_endian_t``]) [ type_of_bil_imm_def, size_of_bil_immtype_def, bil_number_of_mem_splits_REWRS, bil_store_in_mem_REWRS, thm_prune2]
+     thm0
+
+  val thm2 = Ho_Rewrite.REWRITE_RULE [fold_bil_endian_THM] thm1
+
+  val thm3 = SIMP_RULE (list_ss) [
+     FORALL_AND_THM, type_of_bil_imm_def, size_of_bil_immtype_def]
+     thm2
+
+  val thm4 = REWRITE_RULE [b2n_def, GSYM CONJ_ASSOC] (CONJ thm3 thm_prune2)
+in thm4
+end);
+
+
+(* ------------------------------------------------------------------------- *)
+(*  Boolean Expressions                                                      *)
+(* ------------------------------------------------------------------------- *)
+
+val bil_dest_bool_val_def = Define `
+  (bil_dest_bool_val (Imm (Imm1 w)) = SOME (w = 1w)) /\
+  (bil_dest_bool_val _ = NONE)`
+
+val bil_dest_bool_val_EQ_NONE = store_thm ("bil_dest_bool_val_EQ_NONE",
+  ``!v. (bil_dest_bool_val v = NONE) <=> ~(bil_val_is_Bool v)``,
+Cases >> SIMP_TAC std_ss [bil_val_checker_REWRS, bil_dest_bool_val_def] >>
+Cases_on `b` >> SIMP_TAC (std_ss++bil_imm_ss) [bil_val_checker_REWRS, bil_dest_bool_val_def,
+  type_of_bil_imm_def]);
+
+
+
+val _ = export_theory();
