bil_immScript.sml
@@ -1,0 +1,422 @@
+(* ========================================================================= *)
+(* FILE          : bilScript.sml                                             *)
+(* DESCRIPTION   : A model of immediates from BAP Intermediate Language.     *)
+(* AUTHOR        : (c) Thomas Tuerk <tuerk@kth.se> based on previous work    *)
+(*                 by Roberto Metere, KTH - Royal Institute of Technology    *)
+(* DATE          : 2017                                                      *)
+(* ========================================================================= *)
+
+open HolKernel Parse boolLib bossLib;
+open wordsTheory bitstringTheory;
+open bil_auxiliaryTheory;
+
+val _ = new_theory "bil_imm";
+
+(* ------------------------------------------------------------------------- *)
+(*  Immediates                                                               *)
+(* ------------------------------------------------------------------------- *)
+
+(* Bil immediates can be words of various sizes *)
+val _ = Datatype `bil_imm_t =
+    Imm1  bool[1]
+  | Imm8  bool[8]
+  | Imm16 bool[16]
+  | Imm32 bool[32]
+  | Imm64 bool[64]
+`;
+
+
+(* It is handy to keep track of the size via both a special datatype and a number *)
+val _ = Datatype `bil_immtype_t =
+  | Bit1
+  | Bit8
+  | Bit16
+  | Bit32
+  | Bit64
+`;
+
+val bil_imm_ss = rewrites ((type_rws ``:bil_imm_t``) @ (type_rws ``:bil_immtype_t``));
+
+val type_of_bil_imm_def = Define `
+  (type_of_bil_imm (Imm1  _) = Bit1) /\
+  (type_of_bil_imm (Imm8  _) = Bit8) /\
+  (type_of_bil_imm (Imm16 _) = Bit16) /\
+  (type_of_bil_imm (Imm32 _) = Bit32) /\
+  (type_of_bil_imm (Imm64 _) = Bit64)`;
+
+val size_of_bil_immtype_def = Define `
+  (size_of_bil_immtype Bit1  = 1) /\
+  (size_of_bil_immtype Bit8  = 8) /\
+  (size_of_bil_immtype Bit16 = 16) /\
+  (size_of_bil_immtype Bit32 = 32) /\
+  (size_of_bil_immtype Bit64 = 64)`
+
+val bil_immtype_of_size_def = Define `
+  bil_immtype_of_size n = (
+         if n = 1  then SOME Bit1
+    else if n = 8  then SOME Bit8
+    else if n = 16 then SOME Bit16
+    else if n = 32 then SOME Bit32
+    else if n = 64 then SOME Bit64
+    else NONE)`;
+
+val is_valid_bil_immtype_size_def = Define `
+  is_valid_bil_immtype_size n = ?b. n = size_of_bil_immtype b`;
+
+
+(* A few sanity checks *)
+val size_of_bil_immtype_INJ = store_thm ("size_of_bil_immtype_INJ",
+  ``!b1 b2. (size_of_bil_immtype b1 = size_of_bil_immtype b2) <=> (b1 = b2)``,
+Cases >> Cases >> SIMP_TAC (std_ss++bil_imm_ss) [size_of_bil_immtype_def]);
+
+val size_of_bil_immtype_NEQ_0 = store_thm ("size_of_bil_immtype_NEQ_0",
+  ``!b. size_of_bil_immtype b <> 0``,
+Cases >> SIMP_TAC arith_ss [size_of_bil_immtype_def])
+
+val is_valid_bil_immtype_size_REWRS = save_thm ("is_valid_bil_immtype_size_REWRS",
+  SIMP_RULE (std_ss++DatatypeSimps.expand_type_quants_ss [``:bil_immtype_t``]) [size_of_bil_immtype_def] is_valid_bil_immtype_size_def);
+
+val is_valid_bil_immtype_size_IS_SOME = store_thm ("is_valid_bil_immtype_size_IS_SOME",
+  ``!n. is_valid_bil_immtype_size n <=> IS_SOME (bil_immtype_of_size n)``,
+SIMP_TAC std_ss [is_valid_bil_immtype_size_REWRS, bil_immtype_of_size_def] >>
+METIS_TAC[optionTheory.IS_SOME_DEF]);
+
+val bil_immtype_of_num_inv = store_thm ("bil_immtype_of_num_inv",
+  ``(!brt. bil_immtype_of_size (size_of_bil_immtype brt) = SOME brt) /\
+    (!n brt. (bil_immtype_of_size n = SOME brt) ==>
+             (size_of_bil_immtype brt = n))``,
+REPEAT CONJ_TAC >| [
+  Cases >> SIMP_TAC std_ss [size_of_bil_immtype_def, bil_immtype_of_size_def],
+
+  SIMP_TAC (std_ss++boolSimps.LIFT_COND_ss) [bil_immtype_of_size_def, DISJ_IMP_THM, FORALL_AND_THM,
+    COND_EXPAND_OR, LEFT_AND_OVER_OR, size_of_bil_immtype_def]
+]);
+
+
+
+(* ------------------------------------------------------------------------- *)
+(*  Transformation between immediates and numbers                            *)
+(* ------------------------------------------------------------------------- *)
+val b2n_def = Define `
+  (b2n ( Imm1  w ) = w2n w) /\
+  (b2n ( Imm8  w ) = w2n w) /\
+  (b2n ( Imm16 w ) = w2n w) /\
+  (b2n ( Imm32 w ) = w2n w) /\
+  (b2n ( Imm64 w ) = w2n w)
+`;
+
+val n2bs_def = Define `
+  (n2bs n Bit1  = Imm1  (n2w n)) /\
+  (n2bs n Bit8  = Imm8  (n2w n)) /\
+  (n2bs n Bit16 = Imm16 (n2w n)) /\
+  (n2bs n Bit32 = Imm32 (n2w n)) /\
+  (n2bs n Bit64 = Imm64 (n2w n))`
+
+val n2b_1_def  = Define `n2b_1  n = n2bs n Bit1`;
+val n2b_8_def  = Define `n2b_8  n = n2bs n Bit8`;
+val n2b_16_def = Define `n2b_16 n = n2bs n Bit16`;
+val n2b_32_def = Define `n2b_32 n = n2bs n Bit32`;
+val n2b_64_def = Define `n2b_64 n = n2bs n Bit64`;
+
+val _ = add_bare_numeral_form (#"x", SOME "n2b_64");
+val _ = add_bare_numeral_form (#"e", SOME "n2b_32");
+val _ = add_bare_numeral_form (#"d", SOME "n2b_16");
+val _ = add_bare_numeral_form (#"c", SOME "n2b_8");
+val _ = add_bare_numeral_form (#"b", SOME "n2b_1");
+
+val n2b_fixed_DEFS = save_thm ("n2b_fixed_DEFS",
+    LIST_CONJ [n2b_1_def, n2b_8_def, n2b_16_def, n2b_32_def, n2b_64_def]);
+
+val b2n_n2bs = store_thm ("b2n_n2bs",
+  ``!bt n. b2n (n2bs n bt) = MOD_2EXP (size_of_bil_immtype bt) n``,
+Cases >> (
+  SIMP_TAC (std_ss++wordsLib.WORD_ss) [b2n_def, n2bs_def, w2n_n2w,
+    size_of_bil_immtype_def, bitTheory.MOD_2EXP_def]
+));
+
+val b2n_n2b_fixed = store_thm ("b2n_n2b_fixed",
+  ``(!n. b2n (n2b_1 n)  = n MOD 2) /\
+    (!n. b2n (n2b_8 n)  = n MOD 2**8) /\
+    (!n. b2n (n2b_16 n) = n MOD 2**16) /\
+    (!n. b2n (n2b_32 n) = n MOD 2**32) /\
+    (!n. b2n (n2b_64 n) = n MOD 2**64) /\
+    (!n bt. b2n (n2bs n bt) = n MOD 2**(size_of_bil_immtype bt))``,
+
+SIMP_TAC std_ss [n2b_fixed_DEFS, b2n_n2bs, size_of_bil_immtype_def,
+  bitTheory.MOD_2EXP_def]);
+
+val n2bs_b2n = store_thm ("n2bs_b2n",
+  ``!b s. (s = type_of_bil_imm b) ==> (n2bs (b2n b) s = b)``,
+Cases >> (
+  SIMP_TAC std_ss [b2n_def, n2bs_def, type_of_bil_imm_def, n2w_w2n]
+));
+
+
+val w2n_lt_trans = prove (``!w:'a word. dimword (:'a) <= m ==> (w2n w < m)``,
+METIS_TAC[w2n_lt, arithmeticTheory.LESS_LESS_EQ_TRANS]);
+
+val b2n_lt = store_thm ("b2n_lt",
+  ``!b. b2n b < 2 ** (size_of_bil_immtype (type_of_bil_imm b))``,
+Cases >> (
+  SIMP_TAC std_ss [b2n_def, type_of_bil_imm_def, size_of_bil_immtype_def] >>
+  MATCH_MP_TAC w2n_lt_trans >>
+  SIMP_TAC (std_ss++wordsLib.SIZES_ss) []
+));
+
+
+val b2n_lt_REWRS = save_thm ("b2n_lt_REWRS",
+SIMP_RULE (std_ss++DatatypeSimps.expand_type_quants_ss[``:bil_imm_t``]) [
+  type_of_bil_imm_def, size_of_bil_immtype_def] b2n_lt);
+
+
+val b2n_MOD_2EXP = store_thm ("b2n_MOD_2EXP",
+  ``!i n. ((size_of_bil_immtype (type_of_bil_imm i)) = n) ==>
+          (MOD_2EXP n (b2n i) = b2n i)``,
+SIMP_TAC std_ss [bitTheory.MOD_2EXP_def, b2n_lt]);
+
+
+val type_of_n2bs = store_thm ("type_of_n2bs",
+``!s n. type_of_bil_imm (n2bs n s) = s``,
+Cases >> SIMP_TAC std_ss [n2bs_def, type_of_bil_imm_def]);
+
+
+val type_of_n2b_fixed = save_thm ("type_of_n2b_fixed",
+SIMP_RULE (std_ss++DatatypeSimps.expand_type_quants_ss [``:bil_immtype_t``]) [
+  GSYM n2b_fixed_DEFS] type_of_n2bs);
+
+
+val type_of_bil_imm_n2bs_INTRO = store_thm ("type_of_bil_imm_n2bs_INTRO",
+  ``!s b. (type_of_bil_imm b = s) <=> (?n. b = n2bs n s)``,
+
+REPEAT GEN_TAC >> EQ_TAC >> STRIP_TAC >| [
+  Q.EXISTS_TAC `b2n b` >>
+  ASM_SIMP_TAC std_ss [n2bs_b2n],
+
+  ASM_SIMP_TAC std_ss [type_of_n2bs]
+]);
+
+
+
+(* ------------------------------------------------------------------------- *)
+(*  transformation between immediates and words                              *)
+(* ------------------------------------------------------------------------- *)
+
+val b2w_def = Define `b2w bi = n2w (b2n bi)`;
+
+val b2w_REWRS = store_thm ("b2w_REWRS",
+``(!w. (b2w ( Imm1  w ) = w2w w)) /\
+  (!w. (b2w ( Imm8  w ) = w2w w)) /\
+  (!w. (b2w ( Imm16 w ) = w2w w)) /\
+  (!w. (b2w ( Imm32 w ) = w2w w)) /\
+  (!w. (b2w ( Imm64 w ) = w2w w))``,
+REWRITE_TAC[b2w_def, b2n_def, w2w_def]);
+
+val w2bs_def = Define `w2bs w s = n2bs (w2n w) s`
+
+val w2bs_REWRS = store_thm ("w2bs_REWRS",
+``(!w. (w2bs w Bit1  = Imm1  (w2w w))) /\
+  (!w. (w2bs w Bit8  = Imm8  (w2w w))) /\
+  (!w. (w2bs w Bit16 = Imm16 (w2w w))) /\
+  (!w. (w2bs w Bit32 = Imm32 (w2w w))) /\
+  (!w. (w2bs w Bit64 = Imm64 (w2w w)))``,
+SIMP_TAC std_ss [w2bs_def,n2bs_def, w2w_def]);
+
+
+val w2bs_b2w = store_thm ("w2bs_b2w",
+  ``!b s. ((s = type_of_bil_imm b) /\ size_of_bil_immtype (type_of_bil_imm b) <= dimindex (:'a)) ==>
+          (w2bs ((b2w b):'a word) s = b)``,
+SIMP_TAC std_ss [w2bs_def, b2w_def, w2n_n2w] >>
+REPEAT STRIP_TAC >>
+`b2n b MOD (dimword (:'a)) = b2n b` by (
+  MATCH_MP_TAC arithmeticTheory.LESS_MOD >>
+  ASSUME_TAC (Q.SPEC `b` b2n_lt) >>
+  FULL_SIMP_TAC arith_ss [dimword_def] >>
+  `2 ** size_of_bil_immtype (type_of_bil_imm b) <= 2 ** dimindex (:'a)` by
+     METIS_TAC[bitTheory.TWOEXP_MONO2] >>
+  DECIDE_TAC
+) >>
+ASM_SIMP_TAC std_ss [n2bs_b2n])
+
+val type_of_w2bs = store_thm ("type_of_w2bs",
+``!s w. type_of_bil_imm (w2bs w s) = s``,
+SIMP_TAC std_ss [w2bs_def, type_of_n2bs]);
+
+
+(* ------------------------------------------------------------------------- *)
+(*  transformation between immediates and bool                               *)
+(* ------------------------------------------------------------------------- *)
+
+val b2bool_def = Define `b2bool bi = (b2n bi <> 0)`;
+
+val b2bool_REWRS = save_thm ("b2bool_REWRS",
+  SIMP_RULE (std_ss++DatatypeSimps.expand_type_quants_ss[``:bil_imm_t``]) [
+    b2n_def, w2n_eq_0]
+    b2bool_def);
+
+val bool2b_def = Define `bool2b b = if b then Imm1 1w else Imm1 0w`;
+
+val bool2b_inv = store_thm ("bool2b_inv",
+  ``(!b. (b2bool (bool2b b) = b)) /\
+    (!w. ((bool2b (b2bool (Imm1 w))) = Imm1 w))``,
+
+SIMP_TAC (std_ss++boolSimps.LIFT_COND_ss++wordsLib.WORD_ss)
+  [b2bool_def, bool2b_def, b2n_def, w2n_eq_0] >>
+Cases >>
+FULL_SIMP_TAC (std_ss++wordsLib.WORD_ss) [] >>
+`(n = 0) \/ (n = 1)` by DECIDE_TAC >> (
+  ASM_SIMP_TAC std_ss []
+));
+
+val type_of_bool2b = store_thm ("type_of_bool2b",
+  ``!b. type_of_bil_imm (bool2b b) = Bit1``,
+Cases >> SIMP_TAC std_ss [bool2b_def, type_of_bil_imm_def]);
+
+
+(* ------------------------------------------------------------------------- *)
+(*  transformation between immediates and bitstrings                         *)
+(* ------------------------------------------------------------------------- *)
+
+val v2bs_def = Define `v2bs v s = n2bs (v2n v) s`;
+
+val v2bs_REWRS = save_thm ("v2bs_REWRS",
+  SIMP_RULE (std_ss++DatatypeSimps.expand_type_quants_ss[``:bil_immtype_t``]) [
+    n2bs_def, FORALL_AND_THM, n2w_v2n] v2bs_def);
+
+val b2v_def = Define `
+  (b2v ( Imm1  w ) = w2v w) /\
+  (b2v ( Imm8  w ) = w2v w) /\
+  (b2v ( Imm16 w ) = w2v w) /\
+  (b2v ( Imm32 w ) = w2v w) /\
+  (b2v ( Imm64 w ) = w2v w)
+`;
+
+val b2v_LENGTH = store_thm ("b2v_LENGTH",
+  ``!r. LENGTH (b2v r) = size_of_bil_immtype (
+        type_of_bil_imm r)``,
+Cases >> (
+  SIMP_TAC (std_ss++wordsLib.WORD_ss) [b2v_def, type_of_bil_imm_def,
+    size_of_bil_immtype_def, length_w2v]
+));
+
+val v2n_w2v = store_thm ("v2n_w2v",
+``!w:'a word. (v2n (w2v w) = w2n w)``,
+GEN_TAC >>
+bitstringLib.Cases_on_v2w `w` >>
+ASM_SIMP_TAC std_ss [w2n_v2w, w2v_v2w,
+  fixwidth_id_imp, bitTheory.MOD_2EXP_def, v2n_lt]
+);
+
+val v2n_b2v = store_thm ("v2n_b2v",
+  ``!r. v2n (b2v r) = b2n r``,
+Cases >> (
+  SIMP_TAC (std_ss++wordsLib.WORD_ss) [b2n_def, b2v_def, v2n_w2v]
+));
+
+
+val type_of_v2bs = store_thm ("type_of_v2bs",
+``!s v. type_of_bil_imm (v2bs v s) = s``,
+SIMP_TAC std_ss [v2bs_def, type_of_n2bs]);
+
+
+val v2w_fixwidth_imp = store_thm ("v2w_fixwidth_imp",
+  ``!v w. ((dimindex (:'a)) <= w) ==>
+          ((v2w (fixwidth w v) = ((v2w v):'a word)))``,
+REPEAT STRIP_TAC >>
+`fixwidth (dimindex (:'a)) (fixwidth w v) = fixwidth (dimindex (:'a)) v` by (
+  METIS_TAC[fixwidth_fixwidth_le]
+) >>
+METIS_TAC[v2w_fixwidth]);
+
+
+val v2bs_fixwidth = store_thm ("v2bs_fixwidth",
+``!v vty w. (size_of_bil_immtype vty <= w) ==>
+            (v2bs (fixwidth w v) vty = v2bs v vty)``,
+
+GEN_TAC >> Cases >>
+SIMP_TAC (std_ss++wordsLib.WORD_ss) [v2bs_def, n2bs_def, n2w_v2n,
+  v2w_fixwidth_imp, size_of_bil_immtype_def]);
+
+val v2bs_n2v = store_thm ("v2bs_n2v",
+  ``!n. v2bs (n2v n) = n2bs n``,
+SIMP_TAC std_ss [FUN_EQ_THM, v2bs_def, v2n_n2v]);
+
+
+
+val n2v_v2n = store_thm ("n2v_v2n",
+``!v n. (LENGTH v = n) ==> (fixwidth n (n2v (v2n v)) = v)``,
+
+GEN_TAC >>
+SIMP_TAC list_ss [v2n_def, n2v_def, numposrepTheory.num_from_bin_list_def,
+    numposrepTheory.num_to_bin_list_def] >>
+`EVERY ($> 2) (bitify [] v)` by (
+   SIMP_TAC list_ss [bitify_reverse_map, listTheory.EVERY_MEM,
+     listTheory.MEM_MAP, GSYM LEFT_FORALL_IMP_THM] >>
+   Cases >> SIMP_TAC std_ss []
+) >>
+
+FULL_SIMP_TAC list_ss [numposrepTheory.n2l_l2n, numposrepTheory.l2n_eq_0,
+  boolify_reverse_map, bitify_reverse_map, listTheory.EVERY_MEM,
+  listTheory.MEM_MAP, GSYM LEFT_FORALL_IMP_THM] >>
+POP_ASSUM (K ALL_TAC) >>
+SIMP_TAC (list_ss++boolSimps.LIFT_COND_ss) [listTheory.MAP_TAKE,
+  rich_listTheory.MAP_REVERSE, listTheory.MAP_MAP_o, combinTheory.o_DEF,
+  GSYM rich_listTheory.LASTN_def] >>
+COND_CASES_TAC >- (
+  SIMP_TAC list_ss [fixwidth_def, LET_DEF, zero_extend_def,
+    listTheory.PAD_LEFT] >>
+  Cases_on `v` >> FULL_SIMP_TAC list_ss [] >>
+  rename1 `LENGTH v` >>
+  Cases_on `v` >> FULL_SIMP_TAC list_ss [GSYM rich_listTheory.REPLICATE_GENLIST] >>
+  rename1 `LENGTH v` >>
+
+  `[F] = REPLICATE (SUC 0) F` by SIMP_TAC list_ss [rich_listTheory.REPLICATE] >>
+  ASM_REWRITE_TAC[rich_listTheory.REPLICATE_APPEND, arithmeticTheory.ADD_CLAUSES] >>
+  SIMP_TAC list_ss [rich_listTheory.REPLICATE] >>
+  Induct_on `v` >> (
+    ASM_SIMP_TAC list_ss [rich_listTheory.REPLICATE]
+  )
+) >>
+
+
+Q.SUBGOAL_THEN `(LOG 2 (l2n 2 (REVERSE (MAP (\b. if b then 1 else 0) v)))) =
+  PRE (LENGTH (dropWhile ($= 0) (REVERSE (REVERSE (MAP (\b. if b then 1 else 0) v)))))` SUBST1_TAC >- (
+   MATCH_MP_TAC numposrepTheory.LOG_l2n_dropWhile >>
+   ASM_SIMP_TAC list_ss [listTheory.EXISTS_MEM, listTheory.EVERY_MEM,
+     listTheory.MEM_MAP, GSYM LEFT_FORALL_IMP_THM] >>
+   FULL_SIMP_TAC (std_ss++boolSimps.LIFT_COND_ss) [GSYM LEFT_EXISTS_AND_THM] >>
+   Q.EXISTS_TAC `1` >> ASM_SIMP_TAC std_ss []
+) >>
+FULL_SIMP_TAC (list_ss++boolSimps.LIFT_COND_ss) [dropWhile_MAP, combinTheory.o_DEF] >>
+
+Q.SUBGOAL_THEN `(SUC (PRE (LENGTH (dropWhile (\b. ~b) v)))) = (LENGTH (dropWhile (\b. ~b) v))`
+  SUBST1_TAC >- (
+  Cases_on `dropWhile (\b. ~b) v` >> SIMP_TAC list_ss [] >>
+  FULL_SIMP_TAC list_ss [listTheory.dropWhile_eq_nil, listTheory.EVERY_MEM]
+) >>
+POP_ASSUM (K ALL_TAC) >>
+
+SIMP_TAC list_ss [fixwidth_def, LET_DEF, rich_listTheory.LENGTH_LASTN,
+  listTheory.LENGTH_dropWhile_LESS_EQ] >>
+COND_CASES_TAC >| [
+  SIMP_TAC list_ss [zero_extend_def, listTheory.PAD_LEFT,
+    GSYM rich_listTheory.REPLICATE_GENLIST,
+    rich_listTheory.LENGTH_LASTN, listTheory.LENGTH_dropWhile_LESS_EQ] >>
+  POP_ASSUM (K ALL_TAC) >>
+  Induct_on `v` >- SIMP_TAC list_ss [rich_listTheory.REPLICATE, rich_listTheory.LASTN] >>
+  Cases >- (
+    SIMP_TAC list_ss [rich_listTheory.LASTN_CONS, rich_listTheory.REPLICATE] >>
+    `SUC (LENGTH v) = LENGTH (T::v)` by SIMP_TAC list_ss [] >>
+    ASM_REWRITE_TAC[rich_listTheory.LASTN_LENGTH_ID]
+  ) >>
+
+  `LENGTH (dropWhile (\b. ~b) v) <= LENGTH v` by MATCH_ACCEPT_TAC listTheory.LENGTH_dropWhile_LESS_EQ >>
+  ASM_SIMP_TAC list_ss [arithmeticTheory.SUB, rich_listTheory.REPLICATE,
+    rich_listTheory.LASTN_CONS],
+
+
+  `LENGTH (dropWhile (\b. ~b) v) <= LENGTH v` by MATCH_ACCEPT_TAC listTheory.LENGTH_dropWhile_LESS_EQ >>
+  `LENGTH (dropWhile (\b. ~b) v) = LENGTH v` by DECIDE_TAC >>
+  ASM_SIMP_TAC list_ss [rich_listTheory.LASTN_LENGTH_ID]
+]);
+
+val _ = export_theory();
