bil_imm_expScript.sml
@@ -1,0 +1,528 @@
+(* ========================================================================= *)
+(* FILE          : bilScript.sml                                             *)
+(* DESCRIPTION   : A model of immediate expressions                          *)
+(* AUTHOR        : (c) Thomas Tuerk <tuerk@kth.se> based on previous work    *)
+(*                 by Roberto Metere, KTH - Royal Institute of Technology    *)
+(* DATE          : 2017                                                      *)
+(* ========================================================================= *)
+
+open HolKernel Parse boolLib bossLib;
+open wordsTheory bitstringTheory;
+open bil_auxiliaryTheory bil_immTheory;
+
+val _ = new_theory "bil_imm_exp";
+
+val bil_imm_ss = rewrites ((type_rws ``:bil_imm_t``) @ (type_rws ``:bil_immtype_t``));
+
+
+(* ------------------------------------------------------------------------- *)
+(*  Unary expressions                                                        *)
+(* ------------------------------------------------------------------------- *)
+
+val _ = Datatype `bil_unary_exp_t =
+  | ChangeSign
+  | Not`;
+
+val bil_unary_exp_GET_OPER_def = Define
+  `(bil_unary_exp_GET_OPER Not = word_1comp) /\
+   (bil_unary_exp_GET_OPER ChangeSign = word_2comp)`
+
+val bil_unary_exp_def = Define `
+  (bil_unary_exp uo (Imm64 w) = Imm64 (bil_unary_exp_GET_OPER uo w)) /\
+  (bil_unary_exp uo (Imm32 w) = Imm32 (bil_unary_exp_GET_OPER uo w)) /\
+  (bil_unary_exp uo (Imm16 w) = Imm16 (bil_unary_exp_GET_OPER uo w)) /\
+  (bil_unary_exp uo (Imm8 w)  = Imm8  (bil_unary_exp_GET_OPER uo w)) /\
+  (bil_unary_exp uo (Imm1 w)  = Imm1  (bil_unary_exp_GET_OPER uo w))`;
+
+val bil_unary_exp_REWRS = store_thm ("bil_unary_exp_REWRS", ``!uo.
+  (!w. (bil_unary_exp uo (Imm1 w)  = Imm1  (bil_unary_exp_GET_OPER uo w))) /\
+  (!w. (bil_unary_exp uo (Imm8 w)  = Imm8  (bil_unary_exp_GET_OPER uo w))) /\
+  (!w. (bil_unary_exp uo (Imm16 w) = Imm16 (bil_unary_exp_GET_OPER uo w))) /\
+  (!w. (bil_unary_exp uo (Imm32 w) = Imm32 (bil_unary_exp_GET_OPER uo w))) /\
+  (!w. (bil_unary_exp uo (Imm64 w) = Imm64 (bil_unary_exp_GET_OPER uo w)))``,
+SIMP_TAC std_ss [bil_unary_exp_def]);
+
+
+val type_of_bil_unary_exp = store_thm ("type_of_bil_unary_exp",
+  ``!uo r. type_of_bil_imm (bil_unary_exp uo r) = type_of_bil_imm r``,
+GEN_TAC >> Cases >> (
+  SIMP_TAC std_ss [type_of_bil_imm_def, bil_unary_exp_def]
+));
+
+
+(* Instantiate everything *)
+val bil_not_def = Define `bil_not = bil_unary_exp Not`
+val bil_neg_def = Define `bil_neg = bil_unary_exp ChangeSign`
+
+val bil_unary_exps_DEFS = save_thm ("bil_unary_exps_DEFS",
+  LIST_CONJ [bil_not_def, bil_neg_def]);
+
+
+val bil_unary_exp_list = TypeBase.constructors_of ``:bil_unary_exp_t``;
+
+fun inst_CONJ_THM tms thm =
+  REWRITE_RULE [GSYM CONJ_ASSOC] (LIST_CONJ (map (fn t => SPEC t thm) tms));
+
+val type_of_bil_unary_exps = save_thm ("type_of_bil_unary_exps",
+SIMP_RULE (std_ss) [GSYM bil_unary_exps_DEFS] (
+  inst_CONJ_THM bil_unary_exp_list type_of_bil_unary_exp));
+
+val bil_unary_exps_REWRS = save_thm ("bil_unary_exps_REWRS",
+SIMP_RULE std_ss [GSYM bil_unary_exps_DEFS, bil_unary_exp_GET_OPER_def] (
+  inst_CONJ_THM bil_unary_exp_list bil_unary_exp_REWRS));
+
+
+
+(* ------------------------------------------------------------------------- *)
+(*  Binary expressions                                                       *)
+(* ------------------------------------------------------------------------- *)
+
+val _ = Datatype `bil_bin_exp_t =
+  | And
+  | Or
+  | Xor
+  | Plus
+  | Minus
+  | Mult
+  | Div
+  | SignedDiv
+  | Mod
+  | SignedMod
+  | LeftShift
+  | RightShift
+  | SignedRightShift`;
+
+val bil_bin_exp_GET_OPER_def = Define
+  `(bil_bin_exp_GET_OPER And = word_and) /\
+   (bil_bin_exp_GET_OPER Or = word_or) /\
+   (bil_bin_exp_GET_OPER Xor = word_xor) /\
+   (bil_bin_exp_GET_OPER Plus = $+) /\
+   (bil_bin_exp_GET_OPER Minus = $-) /\
+   (bil_bin_exp_GET_OPER Mult = $*) /\
+   (bil_bin_exp_GET_OPER Div = $//) /\
+   (bil_bin_exp_GET_OPER SignedDiv = $/) /\
+   (bil_bin_exp_GET_OPER Mod =  word_mod) /\
+   (bil_bin_exp_GET_OPER SignedMod = word_smod) /\
+   (bil_bin_exp_GET_OPER LeftShift = word_lsl_bv) /\
+   (bil_bin_exp_GET_OPER RightShift = word_lsr_bv) /\
+   (bil_bin_exp_GET_OPER SignedRightShift = word_asr_bv) /\
+   (bil_bin_exp_GET_OPER _ = ARB) (* Should never fire *)`;
+
+val bil_bin_exp_def = Define `
+  (bil_bin_exp uo (Imm64 w1) (Imm64 w2) = Imm64 (bil_bin_exp_GET_OPER uo w1 w2)) /\
+  (bil_bin_exp uo (Imm32 w1) (Imm32 w2) = Imm32 (bil_bin_exp_GET_OPER uo w1 w2)) /\
+  (bil_bin_exp uo (Imm16 w1) (Imm16 w2) = Imm16 (bil_bin_exp_GET_OPER uo w1 w2)) /\
+  (bil_bin_exp uo (Imm8  w1) (Imm8  w2) = Imm8  (bil_bin_exp_GET_OPER uo w1 w2)) /\
+  (bil_bin_exp uo (Imm1  w1) (Imm1  w2) = Imm1  (bil_bin_exp_GET_OPER uo w1 w2)) /\
+  (bil_bin_exp uo _ _ = ARB)`
+
+val bil_bin_exp_REWRS = store_thm ("bil_bin_exp_REWRS", ``!uo.
+  (!w1 w2. (bil_bin_exp uo (Imm64 w1) (Imm64 w2) = Imm64 (bil_bin_exp_GET_OPER uo w1 w2))) /\
+  (!w1 w2. (bil_bin_exp uo (Imm32 w1) (Imm32 w2) = Imm32 (bil_bin_exp_GET_OPER uo w1 w2))) /\
+  (!w1 w2. (bil_bin_exp uo (Imm16 w1) (Imm16 w2) = Imm16 (bil_bin_exp_GET_OPER uo w1 w2))) /\
+  (!w1 w2. (bil_bin_exp uo (Imm8  w1) (Imm8  w2) = Imm8  (bil_bin_exp_GET_OPER uo w1 w2))) /\
+  (!w1 w2. (bil_bin_exp uo (Imm1  w1) (Imm1  w2) = Imm1  (bil_bin_exp_GET_OPER uo w1 w2))) /\
+  (!r1 r2. (type_of_bil_imm r1 <> type_of_bil_imm r2) ==>
+           (bil_bin_exp uo r1 r2 = ARB))``,
+
+GEN_TAC >>
+SIMP_TAC std_ss [bil_bin_exp_def] >>
+REPEAT Cases >> (
+  SIMP_TAC std_ss [bil_bin_exp_def, type_of_bil_imm_def]
+));
+
+val type_of_bil_bin_exp = store_thm ("type_of_bil_bin_exp",
+  ``!oper_r r1 r2. (type_of_bil_imm r1 = type_of_bil_imm r2) ==>
+    (type_of_bil_imm (bil_bin_exp oper_r r1 r2) = type_of_bil_imm r1)``,
+REPEAT Cases >>
+SIMP_TAC (srw_ss()) [type_of_bil_imm_def, bil_bin_exp_REWRS])
+
+
+val bil_add_def  = Define `bil_add  = bil_bin_exp Plus`;
+val bil_sub_def  = Define `bil_sub  = bil_bin_exp Minus`;
+val bil_mul_def  = Define `bil_mul  = bil_bin_exp Mult`;
+val bil_div_def  = Define `bil_div  = bil_bin_exp Div`;
+val bil_sdiv_def = Define `bil_sdiv = bil_bin_exp SignedDiv`;
+val bil_mod_def  = Define `bil_mod  = bil_bin_exp Mod`
+val bil_smod_def = Define `bil_smod = bil_bin_exp SignedMod`
+val bil_lsl_def  = Define `bil_lsl  = bil_bin_exp LeftShift`
+val bil_lsr_def  = Define `bil_lsr  = bil_bin_exp RightShift`
+val bil_asr_def  = Define `bil_asr  = bil_bin_exp SignedRightShift`
+val bil_and_def  = Define `bil_and  = bil_bin_exp And`
+val bil_or_def   = Define `bil_or   = bil_bin_exp Or`
+val bil_xor_def  = Define `bil_xor  = bil_bin_exp Xor`;
+
+val bil_bin_exps_DEFS = save_thm ("bil_bin_exps_DEFS",
+  LIST_CONJ [bil_add_def, bil_sub_def, bil_mul_def, bil_div_def, bil_sdiv_def,
+     bil_mod_def, bil_smod_def, bil_lsl_def, bil_lsr_def, bil_asr_def, bil_and_def,
+     bil_or_def, bil_xor_def]);
+
+val _ = add_infix("<<",  680, HOLgrammars.LEFT);
+val _ = add_infix(">>",  680, HOLgrammars.LEFT);
+val _ = add_infix(">>>", 680, HOLgrammars.LEFT);
+val _ = set_fixity "//" (Infixl 600);
+val _ = set_fixity "/"  (Infixl 600);
+
+val _ = overload_on ("+",              Term`$bil_add`);
+val _ = overload_on ("-",              Term`$bil_sub`);
+val _ = overload_on ("*",              Term`$bil_mul`);
+val _ = overload_on ("//",             Term`$bil_div`);
+val _ = overload_on ("/",              Term`$bil_sdiv`);
+val _ = overload_on ("<<",             Term`$bil_lsl`);
+val _ = overload_on (">>>",            Term`$bil_lsr`);
+val _ = overload_on (">>",             Term`$bil_asr`);
+
+
+val bil_bin_exp_list = TypeBase.constructors_of ``:bil_bin_exp_t``;
+
+val type_of_bil_bin_exps = save_thm ("type_of_bil_bin_exps",
+REWRITE_RULE [GSYM bil_bin_exps_DEFS] (
+  inst_CONJ_THM bil_bin_exp_list type_of_bil_bin_exp));
+
+val bil_bin_exps_REWRS = save_thm ("bil_bin_exps_REWRS",
+SIMP_RULE (std_ss) [GSYM bil_bin_exps_DEFS, bil_bin_exp_GET_OPER_def] (
+  inst_CONJ_THM bil_bin_exp_list bil_bin_exp_REWRS));
+
+
+(* ------------------------------------------------------------------------- *)
+(*  Binary predicates                                                        *)
+(* ------------------------------------------------------------------------- *)
+
+val _ = Datatype `bil_bin_pred_t =
+  | Equal
+  | NotEqual
+  | LessThan
+  | SignedLessThan
+  | LessOrEqual
+  | SignedLessOrEqual`;
+
+
+val bil_bin_pred_GET_OPER_def = Define
+  `(bil_bin_pred_GET_OPER Equal = $=) /\
+   (bil_bin_pred_GET_OPER NotEqual = $<>) /\
+   (bil_bin_pred_GET_OPER LessThan = word_lo) /\
+   (bil_bin_pred_GET_OPER SignedLessThan = word_lt) /\
+   (bil_bin_pred_GET_OPER LessOrEqual = word_ls) /\
+   (bil_bin_pred_GET_OPER SignedLessOrEqual = word_le)`
+
+val bil_bin_pred_def = Define `
+  (bil_bin_pred uo (Imm64 w1) (Imm64 w2) = (bil_bin_pred_GET_OPER uo w1 w2)) /\
+  (bil_bin_pred uo (Imm32 w1) (Imm32 w2) = (bil_bin_pred_GET_OPER uo w1 w2)) /\
+  (bil_bin_pred uo (Imm16 w1) (Imm16 w2) = (bil_bin_pred_GET_OPER uo w1 w2)) /\
+  (bil_bin_pred uo (Imm8  w1) (Imm8  w2) = (bil_bin_pred_GET_OPER uo w1 w2)) /\
+  (bil_bin_pred uo (Imm1  w1) (Imm1  w2) = (bil_bin_pred_GET_OPER uo w1 w2)) /\
+  (bil_bin_pred uo _ _ = F)`;
+
+val bil_bin_pred_REWRS = store_thm ("bil_bin_pred_REWRS", ``!uo.
+  (!w1 w2. (bil_bin_pred uo (Imm64 w1) (Imm64 w2) = (bil_bin_pred_GET_OPER uo w1 w2))) /\
+  (!w1 w2. (bil_bin_pred uo (Imm32 w1) (Imm32 w2) = (bil_bin_pred_GET_OPER uo w1 w2))) /\
+  (!w1 w2. (bil_bin_pred uo (Imm16 w1) (Imm16 w2) = (bil_bin_pred_GET_OPER uo w1 w2))) /\
+  (!w1 w2. (bil_bin_pred uo (Imm8  w1) (Imm8  w2) = (bil_bin_pred_GET_OPER uo w1 w2))) /\
+  (!w1 w2. (bil_bin_pred uo (Imm1  w1) (Imm1  w2) = (bil_bin_pred_GET_OPER uo w1 w2))) /\
+  (!r1 r2. (type_of_bil_imm r1 <> type_of_bil_imm r2) ==>
+     (bil_bin_pred uo r1 r2 = F))``,
+
+GEN_TAC >>
+SIMP_TAC std_ss [bil_bin_pred_def] >>
+REPEAT Cases >> (
+  SIMP_TAC (srw_ss()) [type_of_bil_imm_def, bil_bin_pred_def]
+));
+
+val bil_eq_def  = Define `bil_eq  = bil_bin_pred Equal`
+val bil_neq_def = Define `bil_neq = bil_bin_pred NotEqual`
+val bil_lt_def  = Define `bil_lt  = bil_bin_pred SignedLessThan`
+val bil_le_def  = Define `bil_le  = bil_bin_pred SignedLessOrEqual`
+val bil_ult_def = Define `bil_ult = bil_bin_pred LessThan`
+val bil_ule_def = Define `bil_ule = bil_bin_pred LessOrEqual`
+
+val bil_bin_preds_DEFS = save_thm ("bil_bin_preds_DEFS",
+  LIST_CONJ [bil_eq_def, bil_neq_def, bil_lt_def, bil_le_def, bil_ult_def,
+     bil_ule_def]);
+
+val _ = overload_on ("<",              Term`$bil_lt`);
+val _ = overload_on ("<=",             Term`$bil_le`);
+
+
+val bil_bin_pred_list = TypeBase.constructors_of ``:bil_bin_pred_t``;
+
+val bil_bin_preds_REWRS = save_thm ("bil_bin_preds_REWRS",
+SIMP_RULE (std_ss) [GSYM bil_bin_preds_DEFS, bil_bin_pred_GET_OPER_def] (
+  inst_CONJ_THM bil_bin_pred_list bil_bin_pred_REWRS));
+
+
+
+(* ------------------------------------------------------------------------- *)
+(*  Casts                                                                    *)
+(* ------------------------------------------------------------------------- *)
+
+(* ============= *)
+(* Cast          *)
+(* ============= *)
+
+val bil_cast_def = Define `bil_cast r s = n2bs (b2n r) s`
+
+val bil_cast_REWRS = store_thm ("bil_cast_REWRS", ``
+     (!w. bil_cast (Imm1  w) Bit1  = Imm1  w)
+  /\ (!w. bil_cast (Imm8  w) Bit8  = Imm8  w)
+  /\ (!w. bil_cast (Imm16 w) Bit16 = Imm16 w)
+  /\ (!w. bil_cast (Imm32 w) Bit32 = Imm32 w)
+  /\ (!w. bil_cast (Imm64 w) Bit64 = Imm64 w)
+
+  (* Casts *)
+  /\ (!w. bil_cast (Imm1  w) Bit8  = Imm8  (w2w w))
+  /\ (!w. bil_cast (Imm1  w) Bit16 = Imm16 (w2w w))
+  /\ (!w. bil_cast (Imm1  w) Bit32 = Imm32 (w2w w))
+  /\ (!w. bil_cast (Imm1  w) Bit64 = Imm64 (w2w w))
+  /\ (!w. bil_cast (Imm8  w) Bit1  = Imm1  (w2w w))
+  /\ (!w. bil_cast (Imm8  w) Bit16 = Imm16 (w2w w))
+  /\ (!w. bil_cast (Imm8  w) Bit32 = Imm32 (w2w w))
+  /\ (!w. bil_cast (Imm8  w) Bit64 = Imm64 (w2w w))
+  /\ (!w. bil_cast (Imm16 w) Bit1  = Imm1  (w2w w))
+  /\ (!w. bil_cast (Imm16 w) Bit8  = Imm8  (w2w w))
+  /\ (!w. bil_cast (Imm16 w) Bit32 = Imm32 (w2w w))
+  /\ (!w. bil_cast (Imm16 w) Bit64 = Imm64 (w2w w))
+  /\ (!w. bil_cast (Imm32 w) Bit1  = Imm1  (w2w w))
+  /\ (!w. bil_cast (Imm32 w) Bit8  = Imm8  (w2w w))
+  /\ (!w. bil_cast (Imm32 w) Bit16 = Imm16 (w2w w))
+  /\ (!w. bil_cast (Imm32 w) Bit64 = Imm64 (w2w w))
+  /\ (!w. bil_cast (Imm64 w) Bit1  = Imm1  (w2w w))
+  /\ (!w. bil_cast (Imm64 w) Bit8  = Imm8  (w2w w))
+  /\ (!w. bil_cast (Imm64 w) Bit16 = Imm16 (w2w w))
+  /\ (!w. bil_cast (Imm64 w) Bit32 = Imm32 (w2w w))
+``,
+SIMP_TAC std_ss [bil_cast_def, b2n_def, n2bs_def, GSYM w2w_def, w2w_id])
+
+
+(* ============= *)
+(* lcast         *)
+(* ============= *)
+
+val bil_lcast_def = Define `bil_lcast = bil_cast`;
+
+val bil_lcast_REWRS = save_thm ("bil_lcast_REWRS",
+  REWRITE_RULE [GSYM bil_lcast_def] bil_cast_REWRS);
+
+
+
+(* ============= *)
+(* hcast         *)
+(* ============= *)
+
+val bil_hcast_def = Define `bil_hcast r s =
+  n2bs (DIV_2EXP ((size_of_bil_immtype (type_of_bil_imm r) - (size_of_bil_immtype s))) (b2n r)) s`;
+
+val w2wh_def = Define `w2wh (w : 'a word) = (word_extract (dimindex (:'a) - 1) (dimindex (:'a) - dimindex (:'b)) w) :'b word`;
+
+val w2wh_id = store_thm ("w2wh_id", ``!w. w2wh (w : 'a word) = w``,
+SIMP_TAC (arith_ss++wordsLib.WORD_ss) [w2wh_def,
+  INST_TYPE [beta |-> alpha] wordsTheory.EXTRACT_ALL_BITS, w2w_id]);
+
+val w2wh_w2w = store_thm ("w2wh_w2w", ``!w.
+  (dimindex (:'a) <= dimindex (:'b)) ==> ((w2wh (w : 'a word) : 'b word) = w2w w)``,
+
+REPEAT STRIP_TAC >>
+`(dimindex (:'a) - dimindex (:'b)) = 0` by DECIDE_TAC >>
+ASM_SIMP_TAC (arith_ss++wordsLib.WORD_ss) [w2wh_def, WORD_w2w_EXTRACT]);
+
+
+val bil_hcast_REWRS0 = store_thm ("bil_hcast_REWRS0", ``
+     (!w. bil_hcast (Imm1  w) Bit1  = Imm1  (w2wh w))
+  /\ (!w. bil_hcast (Imm1  w) Bit8  = Imm8  (w2wh w))
+  /\ (!w. bil_hcast (Imm1  w) Bit16 = Imm16 (w2wh w))
+  /\ (!w. bil_hcast (Imm1  w) Bit32 = Imm32 (w2wh w))
+  /\ (!w. bil_hcast (Imm1  w) Bit64 = Imm64 (w2wh w))
+  /\ (!w. bil_hcast (Imm8  w) Bit1  = Imm1  (w2wh w))
+  /\ (!w. bil_hcast (Imm8  w) Bit8  = Imm8  (w2wh w))
+  /\ (!w. bil_hcast (Imm8  w) Bit16 = Imm16 (w2wh w))
+  /\ (!w. bil_hcast (Imm8  w) Bit32 = Imm32 (w2wh w))
+  /\ (!w. bil_hcast (Imm8  w) Bit64 = Imm64 (w2wh w))
+  /\ (!w. bil_hcast (Imm16 w) Bit1  = Imm1  (w2wh w))
+  /\ (!w. bil_hcast (Imm16 w) Bit8  = Imm8  (w2wh w))
+  /\ (!w. bil_hcast (Imm16 w) Bit16 = Imm16 (w2wh w))
+  /\ (!w. bil_hcast (Imm16 w) Bit32 = Imm32 (w2wh w))
+  /\ (!w. bil_hcast (Imm16 w) Bit64 = Imm64 (w2wh w))
+  /\ (!w. bil_hcast (Imm32 w) Bit1  = Imm1  (w2wh w))
+  /\ (!w. bil_hcast (Imm32 w) Bit8  = Imm8  (w2wh w))
+  /\ (!w. bil_hcast (Imm32 w) Bit16 = Imm16 (w2wh w))
+  /\ (!w. bil_hcast (Imm32 w) Bit32 = Imm32 (w2wh w))
+  /\ (!w. bil_hcast (Imm32 w) Bit64 = Imm64 (w2wh w))
+  /\ (!w. bil_hcast (Imm64 w) Bit1  = Imm1  (w2wh w))
+  /\ (!w. bil_hcast (Imm64 w) Bit8  = Imm8  (w2wh w))
+  /\ (!w. bil_hcast (Imm64 w) Bit16 = Imm16 (w2wh w))
+  /\ (!w. bil_hcast (Imm64 w) Bit32 = Imm32 (w2wh w))
+  /\ (!w. bil_hcast (Imm64 w) Bit64 = Imm64 (w2wh w))
+``,
+
+Q.ABBREV_TAC `MY_POW = \x. 2 ** x` >>
+`MY_POW 0 = 1` by (UNABBREV_ALL_TAC >> ASM_SIMP_TAC std_ss []) >>
+ASM_SIMP_TAC std_ss [bil_hcast_def, bitTheory.DIV_2EXP_def] >>
+ASM_SIMP_TAC (std_ss++bil_imm_ss++wordsLib.WORD_ss) [w2wh_def, n2bs_def,
+  b2n_def, size_of_bil_immtype_def, type_of_bil_imm_def, n2w_w2n] >>
+REPEAT CONJ_TAC >> Cases >> (
+  FULL_SIMP_TAC (std_ss++wordsLib.WORD_ss) [word_extract_mask, w2n_n2w] >>
+  blastLib.BBLAST_TAC >>
+  UNABBREV_ALL_TAC >> BETA_TAC >>
+  ASM_SIMP_TAC arith_ss [bitTheory.BIT_SHIFT_THM4, bitTheory.NOT_BIT_GT_TWOEXP] >>
+  METIS_TAC[]
+));
+
+
+val bil_hcast_REWRS = store_thm ("bil_hcast_REWRS", ``
+  (* Not very casts *)
+     (!w. bil_hcast (Imm1  w) Bit1  = Imm1  w)
+  /\ (!w. bil_hcast (Imm8  w) Bit8  = Imm8  w)
+  /\ (!w. bil_hcast (Imm16 w) Bit16 = Imm16 w)
+  /\ (!w. bil_hcast (Imm32 w) Bit32 = Imm32 w)
+  /\ (!w. bil_hcast (Imm64 w) Bit64 = Imm64 w)
+
+  (* Casts *)
+  /\ (!w. bil_hcast (Imm1  w) Bit8  = Imm8  (w2w w))
+  /\ (!w. bil_hcast (Imm1  w) Bit16 = Imm16 (w2w w))
+  /\ (!w. bil_hcast (Imm1  w) Bit32 = Imm32 (w2w w))
+  /\ (!w. bil_hcast (Imm1  w) Bit64 = Imm64 (w2w w))
+  /\ (!w. bil_hcast (Imm8  w) Bit1  = Imm1  (w2wh w))
+  /\ (!w. bil_hcast (Imm8  w) Bit16 = Imm16 (w2w w))
+  /\ (!w. bil_hcast (Imm8  w) Bit32 = Imm32 (w2w w))
+  /\ (!w. bil_hcast (Imm8  w) Bit64 = Imm64 (w2w w))
+  /\ (!w. bil_hcast (Imm16 w) Bit1  = Imm1  (w2wh w))
+  /\ (!w. bil_hcast (Imm16 w) Bit8  = Imm8  (w2wh w))
+  /\ (!w. bil_hcast (Imm16 w) Bit32 = Imm32 (w2w w))
+  /\ (!w. bil_hcast (Imm16 w) Bit64 = Imm64 (w2w w))
+  /\ (!w. bil_hcast (Imm32 w) Bit1  = Imm1  (w2wh w))
+  /\ (!w. bil_hcast (Imm32 w) Bit8  = Imm8  (w2wh w))
+  /\ (!w. bil_hcast (Imm32 w) Bit16 = Imm16 (w2wh w))
+  /\ (!w. bil_hcast (Imm32 w) Bit64 = Imm64 (w2w w))
+  /\ (!w. bil_hcast (Imm64 w) Bit1  = Imm1  (w2wh w))
+  /\ (!w. bil_hcast (Imm64 w) Bit8  = Imm8  (w2wh w))
+  /\ (!w. bil_hcast (Imm64 w) Bit16 = Imm16 (w2wh w))
+  /\ (!w. bil_hcast (Imm64 w) Bit32 = Imm32 (w2wh w))
+``,
+
+SIMP_TAC (std_ss++wordsLib.WORD_ss) [bil_hcast_REWRS0, w2wh_id,
+ w2wh_w2w]);
+
+
+(* ============= *)
+(* scast         *)
+(* ============= *)
+
+val bil_scast_def = Define `bil_scast r s =
+  n2bs (if (type_of_bil_imm r = Bit1) then (b2n r) else
+     (SIGN_EXTEND (size_of_bil_immtype (type_of_bil_imm r))
+                  (size_of_bil_immtype s) (b2n r))) s`;
+
+val bil_scast_REWRS0 = store_thm ("bil_scast_REWRS0", ``
+     (!w. bil_scast (Imm1  w) Bit1  = Imm1  (w2w w))
+  /\ (!w. bil_scast (Imm1  w) Bit8  = Imm8  (w2w w))
+  /\ (!w. bil_scast (Imm1  w) Bit16 = Imm16 (w2w w))
+  /\ (!w. bil_scast (Imm1  w) Bit32 = Imm32 (w2w w))
+  /\ (!w. bil_scast (Imm1  w) Bit64 = Imm64 (w2w w))
+  /\ (!w. bil_scast (Imm8  w) Bit1  = Imm1  (sw2sw w))
+  /\ (!w. bil_scast (Imm8  w) Bit8  = Imm8  (sw2sw w))
+  /\ (!w. bil_scast (Imm8  w) Bit16 = Imm16 (sw2sw w))
+  /\ (!w. bil_scast (Imm8  w) Bit32 = Imm32 (sw2sw w))
+  /\ (!w. bil_scast (Imm8  w) Bit64 = Imm64 (sw2sw w))
+  /\ (!w. bil_scast (Imm16 w) Bit1  = Imm1  (sw2sw w))
+  /\ (!w. bil_scast (Imm16 w) Bit8  = Imm8  (sw2sw w))
+  /\ (!w. bil_scast (Imm16 w) Bit16 = Imm16 (sw2sw w))
+  /\ (!w. bil_scast (Imm16 w) Bit32 = Imm32 (sw2sw w))
+  /\ (!w. bil_scast (Imm16 w) Bit64 = Imm64 (sw2sw w))
+  /\ (!w. bil_scast (Imm32 w) Bit1  = Imm1  (sw2sw w))
+  /\ (!w. bil_scast (Imm32 w) Bit8  = Imm8  (sw2sw w))
+  /\ (!w. bil_scast (Imm32 w) Bit16 = Imm16 (sw2sw w))
+  /\ (!w. bil_scast (Imm32 w) Bit32 = Imm32 (sw2sw w))
+  /\ (!w. bil_scast (Imm32 w) Bit64 = Imm64 (sw2sw w))
+  /\ (!w. bil_scast (Imm64 w) Bit1  = Imm1  (sw2sw w))
+  /\ (!w. bil_scast (Imm64 w) Bit8  = Imm8  (sw2sw w))
+  /\ (!w. bil_scast (Imm64 w) Bit16 = Imm16 (sw2sw w))
+  /\ (!w. bil_scast (Imm64 w) Bit32 = Imm32 (sw2sw w))
+  /\ (!w. bil_scast (Imm64 w) Bit64 = Imm64 (sw2sw w))
+``,
+SIMP_TAC (std_ss++bil_imm_ss++wordsLib.WORD_ss) [
+  bil_scast_def, n2bs_def, sw2sw_def,
+  size_of_bil_immtype_def, type_of_bil_imm_def, b2n_def, GSYM w2w_def]);
+
+
+val bil_scast_REWRS = store_thm ("bil_scast_REWRS", ``
+  (* Indentity *)
+     (!w. bil_scast (Imm1  w) Bit1  = Imm1  w)
+  /\ (!w. bil_scast (Imm8  w) Bit8  = Imm8  w)
+  /\ (!w. bil_scast (Imm16 w) Bit16 = Imm16 w)
+  /\ (!w. bil_scast (Imm32 w) Bit32 = Imm32 w)
+  /\ (!w. bil_scast (Imm64 w) Bit64 = Imm64 w)
+
+  (* Casts *)
+  /\ (!w. bil_scast (Imm1  w) Bit8  = Imm8  (w2w w))
+  /\ (!w. bil_scast (Imm1  w) Bit16 = Imm16 (w2w w))
+  /\ (!w. bil_scast (Imm1  w) Bit32 = Imm32 (w2w w))
+  /\ (!w. bil_scast (Imm1  w) Bit64 = Imm64 (w2w w))
+  /\ (!w. bil_scast (Imm8  w) Bit1  = Imm1  (sw2sw w))
+  /\ (!w. bil_scast (Imm8  w) Bit16 = Imm16 (sw2sw w))
+  /\ (!w. bil_scast (Imm8  w) Bit32 = Imm32 (sw2sw w))
+  /\ (!w. bil_scast (Imm8  w) Bit64 = Imm64 (sw2sw w))
+  /\ (!w. bil_scast (Imm16 w) Bit1  = Imm1  (sw2sw w))
+  /\ (!w. bil_scast (Imm16 w) Bit8  = Imm8  (sw2sw w))
+  /\ (!w. bil_scast (Imm16 w) Bit32 = Imm32 (sw2sw w))
+  /\ (!w. bil_scast (Imm16 w) Bit64 = Imm64 (sw2sw w))
+  /\ (!w. bil_scast (Imm32 w) Bit1  = Imm1  (sw2sw w))
+  /\ (!w. bil_scast (Imm32 w) Bit8  = Imm8  (sw2sw w))
+  /\ (!w. bil_scast (Imm32 w) Bit16 = Imm16 (sw2sw w))
+  /\ (!w. bil_scast (Imm32 w) Bit64 = Imm64 (sw2sw w))
+  /\ (!w. bil_scast (Imm64 w) Bit1  = Imm1  (sw2sw w))
+  /\ (!w. bil_scast (Imm64 w) Bit8  = Imm8  (sw2sw w))
+  /\ (!w. bil_scast (Imm64 w) Bit16 = Imm16 (sw2sw w))
+  /\ (!w. bil_scast (Imm64 w) Bit32 = Imm32 (sw2sw w))
+``,
+SIMP_TAC (std_ss) [bil_scast_REWRS0, w2w_id, sw2sw_id]);
+
+
+(* ============= *)
+(* combination   *)
+(* ============= *)
+
+val _ = Datatype `bil_cast_t =
+  | UnsignedCast
+  | SignedCast
+  | HighCast
+  | LowCast`;
+
+val bil_gencast_def = Define `
+  (bil_gencast UnsignedCast = bil_cast) /\
+  (bil_gencast SignedCast = bil_scast) /\
+  (bil_gencast HighCast = bil_hcast) /\
+  (bil_gencast LowCast = bil_lcast)`;
+
+val bil_casts_DEFS = save_thm ("bil_casts_DEFS",
+  LIST_CONJ [bil_cast_def, bil_scast_def, bil_hcast_def, bil_lcast_def]);
+
+val bil_casts_REWRS = save_thm ("bil_casts_REWRS",
+  LIST_CONJ [bil_cast_REWRS, bil_scast_REWRS, bil_hcast_REWRS, bil_lcast_REWRS]);
+
+
+val type_of_bil_gencast = store_thm ("type_of_bil_gencast",
+  ``!ct b s. type_of_bil_imm (bil_gencast ct b s) = s``,
+Cases >> SIMP_TAC std_ss [bil_gencast_def, bil_casts_DEFS, type_of_n2bs]);
+
+
+val bil_gencast_ID = store_thm ("bil_gencast_ID",
+  ``!ct b s. (type_of_bil_imm b = s) ==> ((bil_gencast ct b s) = b)``,
+Cases >> Cases >> Cases >> (
+  SIMP_TAC (std_ss++bil_imm_ss) [bil_gencast_def, bil_casts_REWRS, type_of_bil_imm_def]
+));
+
+
+val bil_casts_list = TypeBase.constructors_of ``:bil_cast_t``;
+
+val bil_casts_ID = save_thm ("bil_casts_ID",
+REWRITE_RULE [bil_gencast_def] (
+  inst_CONJ_THM bil_casts_list bil_gencast_ID));
+
+val bil_casts_Bit1 = store_thm ("bil_casts_Bit1",
+  ``!ct b c. (type_of_bil_imm b = Bit1) ==>
+             (bil_gencast ct b c = bil_cast b c)``,
+Cases >> Cases >> Cases >> (
+  SIMP_TAC (std_ss++bil_imm_ss) [bil_casts_REWRS, bil_gencast_def, type_of_bil_imm_def]
+));
+
+
+val _ = export_theory();
