bil_valuesScript.sml
@@ -1,0 +1,174 @@
+(* ========================================================================= *)
+(* FILE          : bil_valuesScript.sml                                      *)
+(* DESCRIPTION   : A model of bil values and types                           *)
+(* AUTHOR        : (c) Thomas Tuerk <tuerk@kth.se> based on previous work    *)
+(*                 by Roberto Metere, KTH - Royal Institute of Technology    *)
+(* DATE          : 2017                                                      *)
+(* ========================================================================= *)
+
+open HolKernel Parse boolLib bossLib;
+open wordsTheory bitstringTheory;
+open bil_auxiliaryTheory bil_immTheory;
+
+val _ = new_theory "bil_values";
+
+val bil_imm_ss = rewrites ((type_rws ``:bil_imm_t``) @ (type_rws ``:bil_immtype_t``));
+
+(* ------------------------------------------------------------------------- *)
+(*  Datatypes                                                                *)
+(* ------------------------------------------------------------------------- *)
+
+val _ = Datatype `bil_val_t =
+    Unknown
+  | Imm bil_imm_t
+  | Mem bil_immtype_t (*Addr-Type*) bil_immtype_t (* value-type *) (num -> num)
+`;
+
+
+val _ = Datatype `bil_type_t =
+    NoType
+  | ImmType bil_immtype_t
+  | MemType bil_immtype_t (* Addr-Type *) bil_immtype_t (* Value-Type *)
+`;
+
+val BoolType_def = Define `BoolType = ImmType Bit1`;
+
+
+val bil_val_ss = rewrites (type_rws ``:bil_val_t``);
+val bil_type_ss = rewrites (type_rws ``:bil_type_t``);
+
+
+(* ------------------------------------------------------------------------- *)
+(*  Checkers for Values                                                      *)
+(* ------------------------------------------------------------------------- *)
+
+val bil_val_is_Unknown_def = Define `bil_val_is_Unknown v = (v = Unknown)`;
+val bil_val_is_Imm_def = Define `bil_val_is_Imm v = ?b. (v = Imm b)`;
+val bil_val_is_Imm_s_def = Define `bil_val_is_Imm_s s v = ?n. (v = Imm (n2bs n s))`;
+val bil_val_is_Bool_def = Define `bil_val_is_Bool = bil_val_is_Imm_s Bit1`;
+val bil_val_is_Mem_def = Define `bil_val_is_Mem v = ?at vt mmap. (v = Mem at vt mmap)`;
+
+val bil_val_checker_DEFS = save_thm ("bil_val_checker_DEFS", LIST_CONJ [
+  bil_val_is_Unknown_def, bil_val_is_Imm_def, bil_val_is_Imm_s_def,
+  bil_val_is_Bool_def, bil_val_is_Mem_def]);
+
+
+val bil_val_is_Imm_s_ALT_DEF = store_thm ("bil_val_is_Imm_s_ALT_DEF",
+``!s v. bil_val_is_Imm_s s v <=>
+  (?b. (v = Imm b) /\ (type_of_bil_imm b = s))``,
+
+Cases_on `v` >> (
+  SIMP_TAC (std_ss ++ bil_val_ss) [bil_val_is_Imm_s_def,
+    type_of_bil_imm_n2bs_INTRO]
+));
+
+
+val bil_val_checker_REWRS = store_thm ("bil_val_checker_REWRS",
+  ``bil_val_is_Unknown Unknown /\
+    (!b. ~bil_val_is_Unknown (Imm b)) /\
+    (!at vt mmap. ~(bil_val_is_Unknown (Mem at vt mmap))) /\
+
+    ~(bil_val_is_Imm Unknown) /\
+    (!b. bil_val_is_Imm (Imm b)) /\
+    (!at vt mmap. ~(bil_val_is_Imm (Mem at vt mmap))) /\
+
+    ~(bil_val_is_Mem Unknown) /\
+    (!b. ~(bil_val_is_Mem (Imm b))) /\
+    (!at vt mmap. (bil_val_is_Mem (Mem at vt mmap))) /\
+
+    (!s. ~(bil_val_is_Imm_s s Unknown)) /\
+    (!s b. bil_val_is_Imm_s s (Imm b) <=> (type_of_bil_imm b = s)) /\
+    (!s at vt mmap. ~(bil_val_is_Imm_s s (Mem at vt mmap))) /\
+
+    (~(bil_val_is_Bool Unknown)) /\
+    (!b. bil_val_is_Bool (Imm b) <=> (type_of_bil_imm b = Bit1)) /\
+    (!at vt mmap. ~(bil_val_is_Bool (Mem at vt mmap)))``,
+
+
+  REWRITE_TAC[bil_val_is_Imm_s_ALT_DEF, bil_val_is_Bool_def] >>
+  SIMP_TAC (std_ss ++ bil_val_ss) [bil_val_checker_DEFS]);
+
+
+val bil_val_is_Imm_s_IMPL = store_thm ("bil_val_is_Imm_s_IMPL",
+  ``!s v. bil_val_is_Imm_s s v ==> bil_val_is_Imm v``,
+SIMP_TAC (std_ss++bil_val_ss) [bil_val_is_Imm_def, bil_val_is_Imm_s_def,
+  GSYM LEFT_FORALL_IMP_THM]);
+
+val bil_val_is_Bool_IMPL = store_thm ("bil_val_is_Bool_IMPL",
+  ``!v. bil_val_is_Bool v ==> bil_val_is_Imm v``,
+SIMP_TAC (std_ss++bil_val_ss) [bil_val_is_Imm_def, bil_val_is_Bool_def,
+  bil_val_is_Imm_s_def, GSYM LEFT_FORALL_IMP_THM]);
+
+
+
+(* ------------------------------------------------------------------------- *)
+(*  Some basic typing                                                        *)
+(* ------------------------------------------------------------------------- *)
+
+val type_of_bil_val_def = Define `
+  (type_of_bil_val Unknown = NoType) /\
+  (type_of_bil_val (Imm imm) = ImmType (type_of_bil_imm imm)) /\
+  (type_of_bil_val (Mem at vt _) = MemType at vt)`;
+
+val bil_type_is_NoType_def = Define `bil_type_is_NoType ty = (ty = NoType)`
+val bil_type_is_ImmType_def = Define `bil_type_is_ImmType ty = (?s. ty = ImmType s)`
+val bil_type_is_ImmType_s_def = Define `bil_type_is_ImmType_s s ty = (ty = ImmType s)`
+val bil_type_is_BoolType_def = Define `bil_type_is_BoolType ty = (ty = ImmType Bit1)`
+val bil_type_is_MemType_def = Define `bil_type_is_MemType ty = (?at vt. ty = MemType at vt)`;
+
+val bil_type_checker_DEFS = save_thm ("bil_type_checker_DEFS", LIST_CONJ [
+  bil_type_is_NoType_def, bil_type_is_ImmType_def, bil_type_is_ImmType_s_def,
+  bil_type_is_BoolType_def, bil_type_is_MemType_def]);
+
+
+val bil_type_checker_REWRS = store_thm ("bil_type_checker_REWRS",
+  ``bil_type_is_NoType NoType /\
+    (!b. ~bil_type_is_NoType (ImmType b)) /\
+    (!at vt. ~(bil_type_is_NoType (MemType at vt))) /\
+
+    ~(bil_type_is_ImmType NoType) /\
+    (!b. bil_type_is_ImmType (ImmType b)) /\
+    (!at vt. ~(bil_type_is_ImmType (MemType at vt))) /\
+
+    ~(bil_type_is_MemType NoType) /\
+    (!b. ~(bil_type_is_MemType (ImmType b))) /\
+    (!at vt. (bil_type_is_MemType (MemType at vt))) /\
+
+    (!s. ~(bil_type_is_ImmType_s s NoType)) /\
+    (!s b. bil_type_is_ImmType_s s (ImmType b) <=> (b = s)) /\
+    (!s at vt. ~(bil_type_is_ImmType_s s (MemType at vt))) /\
+
+    (~(bil_type_is_BoolType NoType)) /\
+    (!b. bil_type_is_BoolType (ImmType b) <=> (b = Bit1)) /\
+    (!at vt. ~(bil_type_is_BoolType (MemType at vt)))``,
+
+  SIMP_TAC (std_ss ++ bil_type_ss) [bil_type_checker_DEFS]);
+
+
+val bil_type_is_ImmType_s_IMPL = store_thm ("bil_type_is_ImmType_s_IMPL",
+  ``!s v. bil_type_is_ImmType_s s v ==> bil_type_is_ImmType v``,
+SIMP_TAC (std_ss++bil_type_ss) [bil_type_is_ImmType_def, bil_type_is_ImmType_s_def]);
+
+
+val bil_type_is_BoolType_IMPL = store_thm ("bil_type_is_BoolType_IMPL",
+  ``!v. bil_type_is_BoolType v ==> bil_type_is_ImmType v``,
+SIMP_TAC (std_ss++bil_type_ss) [bil_type_is_ImmType_def, bil_type_is_BoolType_def]);
+
+
+val bil_type_check_bil_type_of_bil_val = store_thm ("bil_type_check_bil_type_of_bil_val",
+  ``(!v. (bil_type_is_NoType (type_of_bil_val v) <=> bil_val_is_Unknown v)) /\
+
+    (!v. (bil_type_is_ImmType (type_of_bil_val v) <=> bil_val_is_Imm v)) /\
+    (!v s. (bil_type_is_ImmType_s s (type_of_bil_val v) <=> bil_val_is_Imm_s s v)) /\
+    (!v. (bil_type_is_BoolType (type_of_bil_val v) <=> bil_val_is_Bool v)) /\
+    (!v. (bil_type_is_MemType (type_of_bil_val v) <=> bil_val_is_Mem v))``,
+
+REPEAT STRIP_TAC >> Cases_on `v` >> (
+  SIMP_TAC std_ss [bil_val_checker_REWRS, bil_type_checker_REWRS,
+    type_of_bil_val_def]
+));
+
+
+
+
+val _ = export_theory();
